logrel init

theories/gitree/reductions.v
@@ -1,6 +1,6 @@
 From iris.proofmode Require Import classes tactics.
 From iris.base_logic.lib Require Export invariants.
-From iris.algebra Require Import list.
+From iris.algebra Require Import list vector.
 From iris.bi.lib Require Import fixpoint.
 From gitrees Require Import prelude.
 From gitrees.gitree Require Import core reify.
@@ -383,10 +383,26 @@ Section internal_step.
     solve_proper.
   Qed.
 
+  Global Instance tp_internal_steps_pre_proper : ∀ Φ,
+    Proper ((≡) ==> (≡)) Φ → Proper ((≡) ==> (≡)) (tp_internal_steps_pre Φ).
+  Proof.
+    intros Φ HΦ.
+    intros [x1 [x2 [x3 [x4 x5]]]] [y1 [y2 [y3 [y4 y5]]]].
+    intros [H1 [H2 [H3 [H4 H5]]]].
+    simpl in *.
+    solve_proper.
+  Qed.
+
   Global Instance tp_internal_steps'_ne : NonExpansive tp_internal_steps'.
   Proof.
     apply least_fixpoint_ne'.
     apply _.
+  Qed.
+
+  Global Instance tp_internal_steps'_proper : Proper ((≡) ==> (≡)) tp_internal_steps'.
+  Proof.
+    apply least_fixpoint_proper.
+    solve_proper.
   Qed.
 
   Global Instance tp_internal_steps_mono : BiMonoPred tp_internal_steps_pre.
@@ -624,6 +640,19 @@ Section internal_step.
     - iExists σ'; iRight; by iExists en.
   Qed.
 
+  Local Lemma internal_step_safe_disj'' α σ β σ' en :
+    (internal_step α σ β σ' en)
+    ⊢ (α ≡ Tick β ∧ σ ≡ σ')
+      ∨ ((∃ op i k, α ≡ Vis op i k ∧ reify r α σ ≡ (σ', Tick β, en))).
+  Proof.
+    rewrite /internal_step /=.
+    iIntros "[(H1 & H2 & H3) | (%op & %i & %k & H)]".
+    - iLeft; by iFrame.
+    - iRight.
+      iExists op, i, k.
+      done.
+  Qed.
+
   Lemma internal_step_tp_internal_step α β σ σ' e1 e2 l
     : ⊢ internal_step α σ β σ' l
       → tp_internal_step (e1 ++ α :: e2) σ (e1 ++ β :: e2 ++ l) σ'.
@@ -675,6 +704,485 @@ Section internal_step.
     - pose proof (effect_safe_externalize _ _ H) as [β [σ' [en G]]].
       by exists β, σ', en.
   Qed.
+
+  (* Local Lemma internal_step_safe_disj''' r α σ β σ' en : *)
+  (*   (internal_step α σ β σ' en) *)
+  (*   ⊢ (∃ β σ', α ≡ Tick β ∧ σ ≡ σ') *)
+  (*     ∨ ((∃ op i k, α ≡ Vis op i k ∧ reify r α σ ≡ (σ', Tick β, en))). *)
+  (* Proof. *)
+  (*   rewrite -bi.or_exist. *)
+  (*   apply bi.exist_mono=>β. *)
+  (*   rewrite -bi.or_exist. *)
+  (*   rewrite /internal_step /=. *)
+  (*   iIntros "(%σ' & %en & [(H1 & H2 & H3) | H])". *)
+  (*   - iExists σ'; iLeft; by iFrame. *)
+  (*   - iExists σ'; iRight; by iExists en. *)
+  (* Qed. *)
+
+  (* Lemma sdfsddfds α σ β st' k' *)
+  (*   (Hdisj : ∀ P Q, disjunction_property P Q) : *)
+  (*   (⊢ tp_internal_steps α σ β st' k') *)
+  (*   → (tp_external_steps r α σ β st' k'). *)
+  (* Proof. *)
+  (*   (* revert α β σ st'. *) *)
+  (*   (* induction k' as [| IH]; intros α β σ σ'. *) *)
+  (*   intros H. *)
+  (*   rewrite tp_internal_steps_unfold in H. *)
+  (*   apply Hdisj in H. *)
+  (*   destruct H. *)
+  (*   - pose proof H as H'. *)
+  (*     rewrite bi.and_elim_l in H'. *)
+  (*     apply uPred.internal_eq_soundness in H'. *)
+  (*     rewrite H'. clear H'. *)
+  (*     pose proof H as H'. *)
+  (*     rewrite bi.and_elim_r in H'. *)
+  (*     pose proof H' as H''. *)
+  (*     rewrite bi.and_elim_l in H'. *)
+  (*     rewrite bi.and_elim_r in H''. *)
+  (*     apply uPred.internal_eq_soundness in H'. *)
+  (*     apply uPred.internal_eq_soundness in H''. *)
+  (*     rewrite H' H''. *)
+  (*     by constructor. *)
+  (*   - admit. *)
+
+  (* α ≡ α0 ++ γ :: α1 ∧ β ≡ α0 ++ γ' :: α1 ++ en ∧ internal_step γ σ γ' σ' en *)
+  (* Local Lemma tp_internal_step_safe_disj α σ : *)
+  (*   (∃ β σ', tp_internal_step α σ β σ') *)
+  (*   ⊢ (∃ β σ', α ≡ Tick β ∧ σ ≡ σ') *)
+  (*     ∨ (∃ β σ' en, (∃ op i k, α ≡ Vis op i k ∧ reify r α σ ≡ (σ', Tick β, en))). *)
+  (* Proof. *)
+  (*   rewrite -bi.or_exist. *)
+  (*   apply bi.exist_mono=>β. *)
+  (*   rewrite -bi.or_exist. *)
+  (*   rewrite /internal_step /=. *)
+  (*   iIntros "(%σ' & %en & [(H1 & H2 & H3) | H])". *)
+  (*   - iExists σ'; iLeft; by iFrame. *)
+  (*   - iExists σ'; iRight; by iExists en. *)
+  (* Qed. *)
+
+  (* Lemma tp_internal_step_safe_tp_external_step α σ : *)
+  (*   (∀ P Q, disjunction_property P Q) → *)
+  (*   (⊢ ∃ β σ', tp_internal_step α σ β σ') → ∃ β σ', tp_external_step r α σ β σ'. *)
+  (* Proof. *)
+  (*   intros Hdisj. *)
+  (*   rewrite internal_step_safe_disj. *)
+  (*   intros [H|H]%Hdisj. *)
+  (*   - pose proof (tick_safe_externalize _ _ H) as [β [σ' G]]. *)
+  (*     by exists β, σ', []. *)
+  (*   - pose proof (effect_safe_externalize _ _ H) as [β [σ' [en G]]]. *)
+  (*     by exists β, σ', en. *)
+  (* Qed. *)
+
+  Local Lemma tick_safe_externalize_model (α : IT) σ :
+    (∃ β σ', α ≡ Tick β ∧ σ ≡ σ' : iProp) -∗ ⌜∃ β σ', external_step r α σ β σ' []⌝.
+  Proof.
+    iIntros "H".
+    destruct (IT_dont_confuse α)
+      as [[e Ha] | [[n Ha] | [ [g Ha] | [[α' Ha]|[op [i [k Ha]]]] ]]].
+    + iExFalso.
+      iDestruct "H" as (β σ') "[Ha Hs]". rewrite Ha.
+      iApply (IT_tick_err_ne). iApply internal_eq_sym.
+      by iApply "Ha".
+    + iExFalso.
+      iDestruct "H" as (β σ') "[Ha Hs]". rewrite Ha.
+      iApply (IT_ret_tick_ne with "Ha").
+    + iExFalso.
+      iDestruct "H" as (β σ') "[Ha Hs]". rewrite Ha.
+      iApply (IT_fun_tick_ne with "Ha").
+    + iExists α', σ. iPureIntro. by econstructor; eauto.
+    + iExFalso.
+      iDestruct "H" as (β σ') "[Ha Hs]". rewrite Ha.
+      iApply (IT_tick_vis_ne). by iApply (internal_eq_sym with "Ha").
+  Qed.
+
+  (* ctx-free steps *)
+  Local Lemma effect_safe_externalize_model (α : IT) σ :
+    (∃ β σ' en, (∃ op i k, α ≡ Vis op i k ∧ reify r α σ ≡ (σ', Tick β, en)) : iProp) -∗
+    ⌜∃ β σ' en, external_step r α σ β σ' en⌝.
+  Proof.
+    iIntros "H".
+    destruct (IT_dont_confuse α)
+      as [[e Ha] | [[n Ha] | [ [g Ha] | [[α' Ha]|[op [i [k Ha]]]] ]]].
+    + iExFalso.
+      iDestruct "H" as (β σ' en op i k) "[Ha _]". rewrite Ha.
+      iApply (IT_vis_err_ne). iApply internal_eq_sym.
+      by iApply "Ha".
+    + iExFalso.
+      iDestruct "H" as (β σ' en op i k) "[Ha _]". rewrite Ha.
+      iApply (IT_ret_vis_ne with "Ha").
+    + iExFalso.
+      iDestruct "H" as (β σ' en op i k) "[Ha _]". rewrite Ha.
+      iApply (IT_fun_vis_ne with "Ha").
+    + iExFalso.
+      iDestruct "H" as (β σ' en op i k) "[Ha _]". rewrite Ha.
+      iApply (IT_tick_vis_ne with "Ha").
+    + destruct (reify r (Vis op i k) σ) as [[σ1 α1] en] eqn:Hr.
+      assert ((∃ α' : IT, α1 ≡ Tick α') ∨ (α1 ≡ Err RuntimeErr)) as [[α' Ha']| Ha'].
+      { eapply (reify_is_always_a_tick r op i k σ).
+        by rewrite Hr.
+      }
+      * iExists α',σ1, en.
+        iPureIntro.
+        eapply external_step_reify; eauto.
+        rewrite -Ha' -Hr; repeat f_equiv; eauto.
+      * iExFalso.
+        iDestruct "H" as (β σ' en' op' i' k') "[_ Hb]".
+        assert (reify r (Vis op i k) σ ≡ reify r α σ) as Har.
+        { f_equiv. by rewrite Ha. }
+        iEval (rewrite -Har) in "Hb".
+        iEval (rewrite Hr) in "Hb".
+        iPoseProof (prod_equivI with "Hb") as "[Hb'' Hb']".
+        iPoseProof (prod_equivI with "Hb''") as "[_ Hb'''']".
+        simpl. rewrite Ha'.
+        iApply (IT_tick_err_ne). iApply (internal_eq_sym with "Hb''''").
+  Qed.
+
+  Lemma internal_step_safe_external_step_model α σ :
+    (∃ β σ' en, internal_step α σ β σ' en) -∗ ⌜∃ β σ' en, external_step r α σ β σ' en⌝.
+  Proof.
+    iIntros "H".
+    iDestruct (internal_step_safe_disj α σ with "H") as "[G|G]".
+    -iPoseProof (tick_safe_externalize_model _ _ with "G") as "(%β & %σ' & %G)".
+      iPureIntro.
+      by exists β, σ', [].
+    - iPoseProof (effect_safe_externalize_model _ _ with "G") as "(%β & %σ' & %en & %G)".
+      iPureIntro.
+      by exists β, σ', en.
+  Qed.
+
+  Local Lemma internal_step_safe_disj' α σ β :
+    (∃ σ' en, internal_step α σ (Ret β) σ' en)
+    ⊢ (∃ σ', α ≡ Tick (Ret β) ∧ σ ≡ σ')
+      ∨ (∃ σ' en, (∃ op i k, α ≡ Vis op i k ∧ reify r α σ ≡ (σ', Tick (Ret β), en))).
+  Proof.
+    rewrite -bi.or_exist.
+    rewrite /internal_step /=.
+    iIntros "(%σ' & %en & [(H1 & H2 & H3) | H])".
+    - iExists σ'; iLeft; by iFrame.
+    - iExists σ'; iRight; by iExists en.
+  Qed.
+
+  Lemma ret_discrete_pure `{!OfeDiscrete A} α (β : A) :
+    (α ≡ Ret (E := F) (A := A) β -∗ ⌜α ≡ Ret β⌝ : iProp).
+  Proof.
+    iIntros "H".
+    destruct (IT_dont_confuse α)
+      as [[e Ha] | [[n Ha] | [ [g Ha] | [[α' Ha]|[op [i [k Ha]]]] ]]].
+    + iExFalso. rewrite Ha.
+      iApply IT_ret_err_ne. iApply internal_eq_sym.
+      by iApply "H".
+    + rewrite Ha.
+      iDestruct (Ret_inj' with "H") as "%K".
+      iPureIntro.
+      by rewrite K.
+    + iExFalso. rewrite Ha.
+      iApply IT_ret_fun_ne. iApply internal_eq_sym.
+      by iApply "H".
+    + iExFalso. rewrite Ha.
+      iApply IT_ret_tick_ne. iApply internal_eq_sym.
+      by iApply "H".
+    + iExFalso. rewrite Ha.
+      iApply IT_ret_vis_ne. iApply internal_eq_sym.
+      by iApply "H".
+  Qed.
+
+  Lemma ret_discrete_pure' α (β : A) :
+    (α ≡ Ret (E := F) (A := A) β -∗ ⌜∃ β, α ≡ Ret β⌝ : iProp).
+  Proof.
+    iIntros "H".
+    destruct (IT_dont_confuse α)
+      as [[e Ha] | [[n Ha] | [ [g Ha] | [[α' Ha]|[op [i [k Ha]]]] ]]].
+    + iExFalso. rewrite Ha.
+      iApply IT_ret_err_ne. iApply internal_eq_sym.
+      by iApply "H".
+    + iExists n.
+      done.
+    + iExFalso. rewrite Ha.
+      iApply IT_ret_fun_ne. iApply internal_eq_sym.
+      by iApply "H".
+    + iExFalso. rewrite Ha.
+      iApply IT_ret_tick_ne. iApply internal_eq_sym.
+      by iApply "H".
+    + iExFalso. rewrite Ha.
+      iApply IT_ret_vis_ne. iApply internal_eq_sym.
+      by iApply "H".
+  Qed.
+
+  Lemma fun_discrete_pure' α β :
+    (α ≡ Fun (E := F) (A := A) β -∗ ⌜∃ β, α ≡ Fun β⌝ : iProp).
+  Proof.
+    iIntros "H".
+    destruct (IT_dont_confuse α)
+      as [[e Ha] | [[n Ha] | [ [g Ha] | [[α' Ha]|[op [i [k Ha]]]] ]]].
+    + iExFalso. rewrite Ha.
+      iApply IT_fun_err_ne. iApply internal_eq_sym.
+      by iApply "H".
+    + iExFalso. rewrite Ha.
+      iApply IT_ret_fun_ne.
+      by iApply "H".
+    + iExists g.
+      done.
+    + iExFalso. rewrite Ha.
+      iApply IT_fun_tick_ne. iApply internal_eq_sym.
+      by iApply "H".
+    + iExFalso. rewrite Ha.
+      iApply IT_fun_vis_ne. iApply internal_eq_sym.
+      by iApply "H".
+  Qed.
+
+  Local Lemma tick_safe_externalize_model' `{!OfeDiscrete A} (α : IT) σ β :
+    (∃ σ', α ≡ Tick (Ret β) ∧ σ ≡ σ' : iProp) -∗ ▷ ⌜∃ σ', external_step r α σ (Ret β) σ' []⌝.
+  Proof.
+    iIntros "H".
+    destruct (IT_dont_confuse α)
+      as [[e Ha] | [[n Ha] | [ [g Ha] | [[α' Ha]|[op [i [k Ha]]]] ]]].
+    + iExFalso.
+      iDestruct "H" as (σ') "[Ha Hs]". rewrite Ha.
+      iApply (IT_tick_err_ne). iApply internal_eq_sym.
+      by iApply "Ha".
+    + iExFalso.
+      iDestruct "H" as (σ') "[Ha Hs]". rewrite Ha.
+      iApply (IT_ret_tick_ne with "Ha").
+    + iExFalso.
+      iDestruct "H" as (σ') "[Ha Hs]". rewrite Ha.
+      iApply (IT_fun_tick_ne with "Ha").
+    + iExists σ.
+      iDestruct "H" as (σ') "[Ha Hs]".
+      iEval (rewrite Ha) in "Ha".
+      iDestruct (Tau_inj' with "Ha") as "J".
+      iDestruct (later_equivI_1 with "J") as "K".
+      iNext.
+      iDestruct (ret_discrete_pure with "K") as "%K".
+      rewrite Ha K.
+      iPureIntro.
+      by constructor.
+    + iExFalso.
+      iDestruct "H" as (σ') "[Ha Hs]". rewrite Ha.
+      iApply (IT_tick_vis_ne). by iApply (internal_eq_sym with "Ha").
+  Qed.
+
+  Local Lemma effect_safe_externalize_model' `{!OfeDiscrete A} (α : IT) σ β :
+    (∃ σ' en, (∃ op i k, α ≡ Vis op i k ∧ reify r α σ ≡ (σ', Tick (Ret β), en)) : iProp) -∗
+    ▷ ⌜∃ σ' en, external_step r α σ (Ret β) σ' en⌝.
+  Proof.
+    iIntros "H".
+    destruct (IT_dont_confuse α)
+      as [[e Ha] | [[n Ha] | [ [g Ha] | [[α' Ha]|[op [i [k Ha]]]] ]]].
+    + iExFalso.
+      iDestruct "H" as (σ' en op i k) "[Ha _]". rewrite Ha.
+      iApply (IT_vis_err_ne). iApply internal_eq_sym.
+      by iApply "Ha".
+    + iExFalso.
+      iDestruct "H" as (σ' en op i k) "[Ha _]". rewrite Ha.
+      iApply (IT_ret_vis_ne with "Ha").
+    + iExFalso.
+      iDestruct "H" as (σ' en op i k) "[Ha _]". rewrite Ha.
+      iApply (IT_fun_vis_ne with "Ha").
+    + iExFalso.
+      iDestruct "H" as (σ' en op i k) "[Ha _]". rewrite Ha.
+      iApply (IT_tick_vis_ne with "Ha").
+    + iDestruct "H" as (σ' en' op' i' k') "[_ #Hb]".
+      assert (reify r (Vis op i k) σ ≡ reify r α σ) as Har.
+      { f_equiv. by rewrite Ha. }
+      destruct (reify r (Vis op i k) σ) as [[σ1 α1] en] eqn:Hr.
+      iAssert ((α1 ≡ Tick (Ret β)))%I as "#H".
+      {
+        rewrite -Har.
+        iPoseProof (prod_equivI with "Hb") as "[Hb'' Hb']".
+        iPoseProof (prod_equivI with "Hb''") as "[_ Hb'''']".
+        iApply "Hb''''".
+      }
+      destruct (IT_dont_confuse α1)
+        as [[e'' Ha''] | [[n'' Ha''] | [ [g'' Ha''] | [[α''' Ha'']|[op'' [i'' [k'' Ha'']]]] ]]].
+      * iExFalso.
+        rewrite Ha''.
+        iDestruct (internal_eq_sym with "H") as "?".
+        iApply IT_tick_err_ne. iAssumption.
+      * iExFalso.
+        rewrite Ha''.
+        iApply IT_ret_tick_ne. iAssumption.
+      * iExFalso.
+        rewrite Ha''.
+        iApply IT_fun_tick_ne. iAssumption.
+      * rewrite Ha''.
+        iNext.
+        iDestruct (ret_discrete_pure with "H") as "%K'".
+        iPureIntro.
+        exists σ1, en.
+        econstructor.
+        ++ apply Ha.
+        ++ rewrite -Har.
+           rewrite Ha''.
+           rewrite K'.
+           done.
+      * iExFalso.
+        rewrite Ha''.
+        iDestruct (internal_eq_sym with "H") as "?".
+        iApply IT_tick_vis_ne. iAssumption.
+  Qed.
+
+  Lemma internal_step_safe_external_step_model' `{!OfeDiscrete A} α σ β :
+    (∃ σ' en, internal_step α σ (Ret β) σ' en)
+    -∗ ▷ ⌜∃ σ' en, external_step r α σ (Ret β) σ' en⌝.
+  Proof.
+    iIntros "H".
+    iDestruct (internal_step_safe_disj' α σ with "H") as "[G|G]".
+    - iPoseProof (tick_safe_externalize_model' _ _ with "G") as ">(%σ' & %G)".
+      iPureIntro.
+      by exists σ', [].
+    - iPoseProof (effect_safe_externalize_model' _ _ with "G") as ">(%σ' & %en & %G)".
+      iPureIntro.
+      by exists σ', en.
+  Qed.
+
+  Lemma tp_internal_step_safe_tp_external_step_model `{!OfeDiscrete A} α σ t :
+    (∃ β σ', tp_internal_step [α] σ (Ret t :: β) σ')
+    -∗ ▷ ⌜∃ β σ', tp_external_step r [α] σ (Ret t :: β) σ'⌝.
+  Proof.
+    iIntros "(%β & %σ' & #H)".
+    iDestruct "H" as "(%α0 & %α1 & %γ & %γ' & %en & #HEQ1 & #HEQ2 & H)".
+    iAssert (α0 ≡ nil ∧ α1 ≡ nil)%I as "(HEQ1' & HEQ2')".
+    {
+      destruct α0 as [| ? α0]; destruct α1 as [| ? α1]; first done; iExFalso.
+      - iDestruct (list_equivI with "HEQ1") as "J".
+        iSpecialize ("J" $! 1).
+        by iDestruct (option_equivI with "J") as "?".
+      - iDestruct (list_equivI with "HEQ1") as "J".
+        iSpecialize ("J" $! 1).
+        destruct α0; simpl; by iDestruct (option_equivI with "J") as "?".
+      - iDestruct (list_equivI with "HEQ1") as "J".
+        iSpecialize ("J" $! 1).
+        destruct α0; simpl; by iDestruct (option_equivI with "J") as "?".
+    }
+    iRewrite "HEQ1'" in "HEQ1"; iRewrite "HEQ1'" in "HEQ2".
+    iRewrite "HEQ2'" in "HEQ1". iRewrite "HEQ2'" in "HEQ2".
+    iSimpl in "HEQ1". iSimpl in "HEQ2".
+    iClear "HEQ1' HEQ2'".
+    iDestruct (list_equivI with "HEQ1") as "J".
+    iSpecialize ("J" $! 0). iSimpl in "J".
+    iDestruct (option_equivI with "J") as "J'".
+    iDestruct (list_equivI with "HEQ2") as "K".
+    iSpecialize ("K" $! 0). iSimpl in "K".
+    iDestruct (option_equivI with "K") as "K'".
+    iClear "HEQ1 J K".
+    iRewrite - "J'" in "H".
+    iRewrite - "K'" in "H".
+
+    iApply (bi.pure_mono (∃ σ' en, external_step r α σ (Ret t) σ' en)).
+    {
+      intros [σ'' [en' H]].
+      exists en', σ''.
+      eapply (tp_external_step_atomic r [α] (Ret t :: en') σ σ'' α (Ret t) [] [] en');
+        [done | done |].
+      apply H.
+    }
+    iClear "HEQ2 J' K'".
+    iApply internal_step_safe_external_step_model'.
+    iExists σ', en.
+    done.
+  Qed.
+
+  (* Lemma tp_internal_steps_safe_tp_external_steps_model *)
+  (*   α σ : *)
+  (*   (∃ t β σ' m, tp_internal_steps α σ (IT_of_V t :: β) σ' m) *)
+  (*   -∗ ▷ ⌜∃ t β σ' m, tp_external_steps r α σ (IT_of_V t :: β) σ' m⌝. *)
+  (* Proof. *)
+  (*   iIntros "(%t & %β & %σ' & %m & H)".     *)
+  (*   iInduction m as [| n IH] "G" forall (α σ). *)
+  (*   - rewrite tp_internal_steps_0. *)
+  (*     iDestruct "H" as "(H1 & H2)".       *)
+  (*     iExists t, β, σ, 0. *)
+  (*     iDestruct (list_equivI with "H1") as "K". *)
+  (*     iSpecialize ("K" $! 0). iSimpl in "K". *)
+  (*     iDestruct (option_equivI with "K") as "K'". *)
+  (*     iDestruct (ret_discrete_pure with "K'") as "%K". *)
+  (*     iNext. *)
+  (*     iPureIntro. *)
+  (*     rewrite K. *)
+  (*     by constructor. *)
+  (*   - rewrite tp_internal_steps_S. *)
+  (*     iDestruct "H" as "(%γ & %σ'' & #H1 & #H2)". *)
+  (*     iSpecialize ("G" $! γ σ'' with "H2"). iClear "H2". *)
+  (*     iDestruct "G" as (β' σ''') ">%G". *)
+  (*     iExists β', σ'''. *)
+
+  (*     iAssert (⌜tp_external_step r α σ γ σ''⌝)%I as "%H2". *)
+  (*     { *)
+
+  (*       admit. *)
+  (*     } *)
+  (*     iNext. *)
+  (*     iPureIntro. *)
+  (*     econstructor; last apply G. *)
+  (*     apply H2. *)
+  (* Admitted. *)
+
+
+  (* Lemma internal_steps_safe_external_steps_model *)
+  (*   `{!OfeDiscrete A} *)
+  (*   α σ β σ' en m : *)
+  (*   (internal_steps α σ (Ret β) σ' en m) *)
+  (*   -∗ ⌜∃ en σ', external_steps r α σ (Ret β) σ' en m⌝. *)
+  (* Proof. *)
+  (*   remember (Ret β) as β'. *)
+  (*   iIntros "H". *)
+  (*   iInduction m as [| n IH] "G" forall (α σ en). *)
+  (*   - rewrite internal_steps_0. *)
+  (*     iDestruct "H" as "(H1 & H2 & H3)". *)
+  (*     rewrite Heqβ'. *)
+  (*     iDestruct (ret_discrete_pure with "H1") as "%K". *)
+  (*     iExists [], σ. *)
+  (*     iPureIntro. *)
+  (*     by constructor. *)
+  (*   - rewrite internal_steps_S. *)
+  (*     iDestruct "H" as (γ σ'' l' l'') "(H1 & H2 & H3)". *)
+  (*     iSpecialize ("G" $! γ σ'' l'' with "H3"). *)
+  (*     iDestruct "G" as (en' σ''') "%H". *)
+  (*     iExists en', σ'''. *)
+
+  (* Lemma tp_internal_steps_safe_tp_external_steps_model *)
+  (*   `{!Inhabited stateO} *)
+  (*   `{!OfeDiscrete A} α σ t m : *)
+  (*   (∃ β σ', tp_internal_steps α σ (Ret t :: β) σ' m) *)
+  (*   -∗ ▷ ⌜∃ β σ', tp_external_steps r α σ (Ret t :: β) σ' m⌝. *)
+  (* Proof. *)
+  (*   iIntros "(%β & %σ' & H)".     *)
+
+  (*   iInduction m as [| n IH] "G" forall (α σ). *)
+  (*   - rewrite tp_internal_steps_0. *)
+  (*     iDestruct "H" as "(H1 & H2)". *)
+  (*     destruct α as [| x α]; *)
+  (*       first by *)
+  (*         ( *)
+  (*           iDestruct (list_equivI with "H1") as "K"; *)
+  (*           iSpecialize ("K" $! 0); iSimpl in "K"; *)
+  (*           iDestruct (option_equivI with "K") as "?" *)
+  (*         ). *)
+  (*     iExists α, σ. *)
+  (*     iDestruct (list_equivI with "H1") as "K". *)
+  (*     iSpecialize ("K" $! 0). iSimpl in "K". *)
+  (*     iDestruct (option_equivI with "K") as "K'". *)
+  (*     iDestruct (ret_discrete_pure with "K'") as "%K". *)
+  (*     iNext. *)
+  (*     iPureIntro. *)
+  (*     rewrite K. *)
+  (*     by constructor. *)
+  (*   - rewrite tp_internal_steps_S. *)
+  (*     iDestruct "H" as "(%γ & %σ'' & #H1 & #H2)".       *)
+  (*     iSpecialize ("G" $! γ σ'' with "H2"). iClear "H2". *)
+  (*     iDestruct "G" as (β' σ''') ">%G". *)
+  (*     iExists β', σ'''. *)
+
+  (*     iAssert (⌜tp_external_step r α σ γ σ''⌝)%I as "%H2". *)
+  (*     { *)
+
+  (*       admit. *)
+  (*     } *)
+  (*     iNext. *)
+  (*     iPureIntro. *)
+  (*     econstructor; last apply G. *)
+  (*     apply H2. *)
+  (* Admitted. *)
 
   Lemma internal_step_ITV α αv β σ σ' en :
     (IT_to_V α ≡ Some αv ⊢ internal_step α σ β σ' en -∗ False : iProp)%I.
@@ -751,6 +1259,1110 @@ Section internal_step.
       iRewrite "Hl".
       iRewrite "Hs2".
       done.
+  Qed.
+
+  Lemma internal_step_safe α σ β σ' en :
+    (⊢ internal_step α σ β σ' en)
+    → (external_step r α σ β σ' en).
+  Proof.
+    intros G.
+    assert (⊢ ▷ internal_step α σ β σ' en) as H.
+    {
+      iStartProof.
+      iPoseProof G as "H".
+      iNext. done.
+    }
+    clear G.
+    destruct (IT_dont_confuse α)
+      as [[e Ha] | [[n Ha] | [ [g Ha] | [[α' Ha]|[op [i [k Ha]]]] ]]].
+    + eapply uPred.pure_soundness.
+      apply uPred.later_soundness in H.
+      iPoseProof H as "H".
+      iExFalso.
+      iApply (internal_step_err σ e β σ' en).
+      iDestruct (internal_eq_rewrite α
+                   (Err e)
+                   (λ a, internal_step a σ β σ' en)%I with "[] H") as "H'".
+      { solve_proper. }
+      { by iPureIntro. }
+      done.
+    + eapply uPred.pure_soundness.
+      apply uPred.later_soundness in H.
+      iPoseProof H as "H".
+      iExFalso.
+      iApply (internal_step_ITV α (RetV n) β σ σ' en with "[] H").
+      iPureIntro.
+      rewrite Ha /=.
+      by rewrite IT_to_V_Ret.
+    + eapply uPred.pure_soundness.
+      apply uPred.later_soundness in H.
+      iPoseProof H as "H".
+      iExFalso.
+      iApply (internal_step_ITV α (FunV g) β σ σ' en with "[] H").
+      iPureIntro.
+      rewrite Ha /=.
+      by rewrite IT_to_V_Fun.
+    + rewrite Ha.
+      cut (⊢@{iProp} ▷ (β ≡ α' ∧ σ ≡ σ' ∧ en ≡ []))%I.
+      {
+        intros G.
+        apply uPred.later_soundness in G.
+        pose proof G as G'.
+        rewrite bi.and_elim_l in G'.
+        apply uPred.internal_eq_soundness in G'.
+        rewrite G'. clear G'.
+        pose proof G as G'.
+        rewrite bi.and_elim_r in G'.
+        rewrite bi.and_elim_l in G'.
+        apply uPred.internal_eq_soundness in G'.
+        rewrite G'. clear G'.
+        pose proof G as G'.
+        rewrite bi.and_elim_r in G'.
+        rewrite bi.and_elim_r in G'.
+        apply uPred.internal_eq_soundness in G'.
+        rewrite G'. clear G'.
+        by econstructor.
+      }
+      apply uPred.later_soundness in H.
+      iPoseProof H as "H".
+      iDestruct (internal_eq_rewrite α
+                   (Tick α')
+                   (λ a, internal_step a σ β σ' en)%I with "[] H") as "H'".
+      { solve_proper. }
+      { by iPureIntro. }
+      iPoseProof (internal_step_tick with "H'") as "(J1 & J2 & J3)".
+      iNext.
+      iFrame "J1 J2 J3".
+    + rewrite Ha.
+      destruct (reify r (Vis op i k) σ) as [[σ1 α1] en'] eqn:Hr.
+      assert ((∃ α1', α1 ≡ Tick α1') ∨ α1 ≡ Err RuntimeErr) as [[α1' Ha']|Ha'].
+      {
+        pose proof (reify_is_always_a_tick r op i k σ α1 σ1 en') as G.
+        apply G.
+        by rewrite Hr.
+      }
+      * cut (⊢@{iProp} ▷ (reify r α σ ≡ (σ', Tick β, en)))%I.
+        {
+          intros G.
+          apply uPred.later_soundness in G.
+          apply uPred.internal_eq_soundness in G.
+          econstructor; first done.
+          rewrite -G.
+          f_equiv.
+          f_equiv.
+          symmetry.
+          apply Ha.
+        }
+        iPoseProof H as "H".
+        iDestruct (internal_eq_rewrite α
+                     (Vis op i k)
+                     (λ a, internal_step a σ β σ' en%I) with "[] H") as "H'".
+        { solve_proper. }
+        { by iPureIntro. }
+        iDestruct (internal_step_vis with "H'") as "H2".
+        iNext.
+        iRewrite - "H2".
+        iPureIntro.
+        do 2 f_equiv.
+        apply Ha.
+      * eapply uPred.pure_soundness.
+        apply uPred.later_soundness in H.
+        iPoseProof H as "H".
+        iDestruct (internal_eq_rewrite α
+                     (Vis op i k)
+                     (λ a, internal_step a σ β σ' en)%I with "[] H") as "H'".
+        { solve_proper. }
+        { by iPureIntro. }
+        iDestruct (internal_step_vis with "H'") as "H2".
+        rewrite Hr Ha'.
+        iExFalso.
+        iDestruct (prod_equivI with "H2") as "(G1 & _)".
+        iDestruct (prod_equivI with "G1") as "(_ & G4)".
+        simpl.
+        iApply IT_tick_err_ne. iApply internal_eq_sym. iAssumption.
+  Qed.
+
+  Lemma internal_step_safe_agnostic α σ :
+    (⊢ ∃ β σ' en, internal_step α σ β σ' en)
+    → (∃ β σ' en, external_step r α σ β σ' en).
+  Proof.
+    intros G.
+    assert (⊢ ▷ ∃ β σ' en, internal_step α σ β σ' en) as H.
+    {
+      iStartProof.
+      iPoseProof G as "H".
+      iNext. done.
+    }
+    clear G.
+    destruct (IT_dont_confuse α)
+      as [[e Ha] | [[n Ha] | [ [g Ha] | [[α' Ha]|[op [i [k Ha]]]] ]]].
+    + eapply uPred.pure_soundness.
+      apply uPred.later_soundness in H.
+      iPoseProof H as "H".
+      iExFalso.
+      iDestruct "H" as (β σ' en) "H".
+      iApply (internal_step_err σ e β σ' en).
+      iDestruct (internal_eq_rewrite α
+                   (Err e)
+                   (λ a, internal_step a σ β σ' en)%I with "[] H") as "H'".
+      { solve_proper. }
+      { by iPureIntro. }
+      done.
+    + eapply uPred.pure_soundness.
+      apply uPred.later_soundness in H.
+      iPoseProof H as "H".
+      iExFalso.
+      iDestruct "H" as (β σ' en) "H".
+      iApply (internal_step_ITV α (RetV n) β σ σ' en with "[] H").
+      iPureIntro.
+      rewrite Ha /=.
+      by rewrite IT_to_V_Ret.
+    + eapply uPred.pure_soundness.
+      apply uPred.later_soundness in H.
+      iPoseProof H as "H".
+      iExFalso.
+      iDestruct "H" as (β σ' en) "H".
+      iApply (internal_step_ITV α (FunV g) β σ σ' en with "[] H").
+      iPureIntro.
+      rewrite Ha /=.
+      by rewrite IT_to_V_Fun.
+    + setoid_rewrite Ha.
+      apply uPred.later_soundness in H.
+      exists α', σ, [].
+      cut (⊢@{iProp} ▷ internal_step (Tick α') σ α' σ []).
+      {
+        intros J.
+        apply uPred.later_soundness in J.
+        by apply internal_step_safe in J.
+      }
+      iPoseProof H as "H".
+      iDestruct "H" as (β σ' en) "H".
+      iDestruct (internal_eq_rewrite α
+                   (Tick α')
+                   (λ a, internal_step a σ β σ' en)%I with "[] H") as "H'".
+      { solve_proper. }
+      { by iPureIntro. }
+      iPoseProof (internal_step_tick with "H'") as "(J1 & J2 & J3)".
+      iNext.
+      iRewrite "J1" in "H".
+      iRewrite - "J2" in "H".
+      iRewrite "J3" in "H".
+      iDestruct (internal_eq_rewrite
+                   α
+                   (Tick α')
+                   (λ a, internal_step a σ α' σ [])%I with "[] H") as "H''".
+      { solve_proper. }
+      { by iPureIntro. }
+      done.
+    + setoid_rewrite Ha.
+      destruct (reify r (Vis op i k) σ) as [[σ1 α1] en'] eqn:Hr.
+      assert ((∃ α1', α1 ≡ Tick α1') ∨ α1 ≡ Err RuntimeErr) as [[α1' Ha']|Ha'].
+      {
+        pose proof (reify_is_always_a_tick r op i k σ α1 σ1 en') as G.
+        apply G.
+        by rewrite Hr.
+      }
+      * cut (⊢@{iProp} ▷ (reify r α σ ≡ (σ1, Tick α1', en')))%I.
+        {
+          intros G.
+          apply uPred.later_soundness in G.
+          apply uPred.internal_eq_soundness in G.
+          exists α1', σ1, en'.
+          econstructor; first done.
+          rewrite -G.
+          f_equiv.
+          f_equiv.
+          symmetry.
+          apply Ha.
+        }
+        iPoseProof H as "H".
+        iNext.
+        iDestruct "H" as (β σ' en) "H".
+        iDestruct (internal_eq_rewrite α
+                     (Vis op i k)
+                     (λ a, internal_step a σ β σ' en%I) with "[] H") as "H'".
+        { solve_proper. }
+        { by iPureIntro. }
+        iDestruct (internal_step_vis with "H'") as "H2".
+        iRewrite - "H2".
+        iPureIntro.
+        assert (reify r (Vis op i k) σ ≡ (σ1, α1, en')) as Hr'.
+        { by rewrite Hr. }
+        rewrite Ha' in Hr'.
+        rewrite -Hr'.
+        do 2 f_equiv.
+        apply Ha.
+      * eapply uPred.pure_soundness.
+        apply uPred.later_soundness in H.
+        iPoseProof H as "H".
+        iDestruct "H" as (β σ' en) "H".
+        iDestruct (internal_eq_rewrite α
+                     (Vis op i k)
+                     (λ a, internal_step a σ β σ' en)%I with "[] H") as "H'".
+        { solve_proper. }
+        { by iPureIntro. }
+        iDestruct (internal_step_vis with "H'") as "H2".
+        rewrite Hr Ha'.
+        iExFalso.
+        iDestruct (prod_equivI with "H2") as "(G1 & _)".
+        iDestruct (prod_equivI with "G1") as "(_ & G4)".
+        simpl.
+        iApply IT_tick_err_ne. iApply internal_eq_sym. iAssumption.
+  Qed.
+
+  Lemma internal_steps_safe α σ β σ' en k :
+    (⊢ internal_steps α σ β σ' en k)
+    → (external_steps r α σ β σ' en k).
+  Proof.
+    intros G.
+    assert (⊢ ▷ internal_steps α σ β σ' en k) as H.
+    {
+      iStartProof.
+      iPoseProof G as "H".
+      iNext. done.
+    }
+    clear G.
+    revert H.
+    revert α β σ σ' en.
+    induction k as [| m IH]; intros α β σ σ' en H.
+    - rewrite internal_steps_0 in H.
+      apply uPred.later_soundness in H.
+
+      pose proof H as H'.
+      rewrite bi.and_elim_l in H'.
+      apply uPred.internal_eq_soundness in H'.
+      rewrite H'; clear H'.
+
+      pose proof H as H'.
+      rewrite bi.and_elim_r in H'.
+      rewrite bi.and_elim_l in H'.
+      apply uPred.internal_eq_soundness in H'.
+      rewrite H'; clear H'.
+
+      pose proof H as H'.
+      rewrite bi.and_elim_r in H'.
+      rewrite bi.and_elim_r in H'.
+      apply uPred.internal_eq_soundness in H'.
+      rewrite H'; clear H'.
+
+      by constructor.
+    - rewrite internal_steps_S in H.
+      destruct (IT_dont_confuse α)
+        as [[e Ha] | [[n Ha] | [ [g Ha] | [[α' Ha]|[op [i [k Ha]]]] ]]].
+      + eapply uPred.pure_soundness.
+        apply uPred.later_soundness in H.
+        iPoseProof H as "H".
+        iDestruct "H" as (γ σ'' l' l'') "(H1 & H2 & H3)".
+        iExFalso.
+        iApply (internal_step_err σ e γ σ'' l').
+        iDestruct (internal_eq_rewrite α
+                     (Err e)
+                     (λ a, internal_step a σ γ σ'' l'%I) with "[] H2") as "H2'".
+        { solve_proper. }
+        { by iPureIntro. }
+        done.
+      + eapply uPred.pure_soundness.
+        apply uPred.later_soundness in H.
+        iPoseProof H as "H".
+        iDestruct "H" as (γ σ'' l' l'') "(H1 & H2 & H3)".
+        iExFalso.
+        iApply (internal_step_ITV α (RetV n) γ σ σ'' l' with "[] H2").
+        iPureIntro.
+        rewrite Ha /=.
+        by rewrite IT_to_V_Ret.
+      + eapply uPred.pure_soundness.
+        apply uPred.later_soundness in H.
+        iPoseProof H as "H".
+        iDestruct "H" as (γ σ'' l' l'') "(H1 & H2 & H3)".
+        iExFalso.
+        iApply (internal_step_ITV α (FunV g) γ σ σ'' l' with "[] H2").
+        iPureIntro.
+        rewrite Ha /=.
+        by rewrite IT_to_V_Fun.
+      + rewrite Ha.
+        eapply (steps_many r _ _ _ _ _ _ [] en en m); first done.
+        * apply external_step_tick; reflexivity.
+        * apply IH.
+          iStartProof.
+          apply uPred.later_soundness in H.
+          iPoseProof H as "H".
+          iDestruct "H" as (γ σ'' l' l'') "(H1 & H2 & H3)".
+          iDestruct (internal_eq_rewrite α
+                     (Tick α')
+                     (λ a, internal_step a σ γ σ'' l'%I) with "[] H2") as "H2'".
+          { solve_proper. }
+          { by iPureIntro. }
+          iClear "H2".
+          iRewrite "H1".
+          iClear "H1". clear H en.
+          iPoseProof (internal_step_tick with "H2'") as "(J1 & J2 & J3)".
+          iRewrite "J2". iRewrite "J3".
+          rewrite app_nil_l.
+          iRewrite "J2" in "H2'".
+          iRewrite "J3" in "H2'".
+          iClear "J2 J3".
+          clear σ l'.
+          iNext.
+          iRewrite - "J1".
+          iApply "H3".
+      + rewrite Ha.
+        destruct (reify r (Vis op i k) σ) as [[σ1 α1] en'] eqn:Hr.
+        assert ((∃ α1', α1 ≡ Tick α1') ∨ α1 ≡ Err RuntimeErr) as [[α1' Ha']|Ha'].
+        {
+          pose proof (reify_is_always_a_tick r op i k σ α1 σ1 en') as G.
+          apply G.
+          by rewrite Hr.
+        }
+        * eapply (steps_many r _ _ _ _ _ _ en' (drop (length en') en) en m).
+          {
+            eapply uPred.internal_eq_soundness.
+            apply uPred.later_soundness in H.
+            iPoseProof H as "H".
+            iDestruct "H" as (γ σ'' l' l'') "(H1 & H2 & H3)".
+            iDestruct (internal_eq_rewrite α
+                         (Vis op i k)
+                         (λ a, internal_step a σ γ σ'' l'%I) with "[] H2") as "H2'".
+            { solve_proper. }
+            { by iPureIntro. }
+            iClear "H2".
+            iDestruct (internal_step_vis with "H2'") as "H2".
+            iClear "H2'".
+            rewrite Hr.
+            iDestruct (prod_equivI with "H2") as "(_ & G2)".
+            simpl.
+            iRewrite "H1".
+            iRewrite - "G2".
+            rewrite drop_app_length.
+            done.
+          }
+          {
+            eapply external_step_reify.
+            - done.
+            - rewrite Hr. rewrite  Ha'. done.
+          }
+          apply IH.
+          apply uPred.later_soundness in H.
+          iPoseProof H as "H".
+          iDestruct "H" as (γ σ'' l' l'') "(H1 & H2 & H3)".
+          iDestruct (internal_eq_rewrite α
+                       (Vis op i k)
+                       (λ a, internal_step a σ γ σ'' l'%I) with "[] H2") as "H2'".
+          { solve_proper. }
+          { by iPureIntro. }
+          iClear "H2".
+          iDestruct (internal_step_vis with "H2'") as "H2".
+          iClear "H2'".
+          rewrite Hr Ha'.
+          iDestruct (prod_equivI with "H2") as "(G1 & G2)".
+          iDestruct (prod_equivI with "G1") as "(G3 & G4)".
+          simpl.
+          iRewrite "G3".
+          iRewrite - "G2" in "H1".
+          iRewrite "H1".
+          iNext.
+          iRewrite "G4".
+          rewrite drop_app drop_all app_nil_l Nat.sub_diag drop_0.
+          done.
+        * eapply uPred.pure_soundness.
+          apply uPred.later_soundness in H.
+          iPoseProof H as "H".
+          iDestruct "H" as (γ σ'' l' l'') "(H1 & H2 & H3)".
+          iDestruct (internal_eq_rewrite α
+                       (Vis op i k)
+                       (λ a, internal_step a σ γ σ'' l'%I) with "[] H2") as "H2'".
+          { solve_proper. }
+          { by iPureIntro. }
+          iClear "H2".
+          iDestruct (internal_step_vis with "H2'") as "H2".
+          iClear "H2'".
+          rewrite Hr Ha'.
+          iExFalso.
+          iDestruct (prod_equivI with "H2") as "(G1 & _)".
+          iDestruct (prod_equivI with "G1") as "(_ & G4)".
+          simpl.
+          iApply IT_tick_err_ne. iApply internal_eq_sym. iAssumption.
+  Qed.
+
+  Lemma internal_steps_safe_agnostic α σ k :
+    (⊢ ∃ β σ' en, internal_steps α σ (IT_of_V β) σ' en k)
+    → (∃ β σ' en, external_steps r α σ (IT_of_V β) σ' en k).
+  Proof.
+    intros G.
+    assert (⊢ ▷ ∃ β σ' en, internal_steps α σ (IT_of_V β) σ' en k) as H.
+    {
+      iStartProof.
+      iPoseProof G as "H".
+      iNext. done.
+    }
+    clear G.
+    revert H.
+    revert α σ.
+    induction k as [| m IH]; intros α σ H.
+    - apply uPred.later_soundness in H.
+      setoid_rewrite internal_steps_0 in H.
+      destruct (IT_to_V α) as [β |] eqn:HEQ.
+      + exists β, σ, [].
+        rewrite IT_of_to_V'; last by rewrite -HEQ.
+        by constructor.
+      + eapply uPred.pure_soundness.
+        iExFalso.
+        iPoseProof H as "H".
+        iDestruct "H" as (β σ' en) "(H1 & H2 & H3)".
+        iAssert (IT_to_V α ≡ IT_to_V (IT_of_V β))%I as "J".
+        { by iApply f_equivI. }
+        rewrite IT_to_of_V.
+        rewrite HEQ.
+        by iDestruct (option_equivI with "J") as "?".
+    - setoid_rewrite internal_steps_S in H.
+      destruct (IT_dont_confuse α)
+        as [[e Ha] | [[n Ha] | [ [g Ha] | [[α' Ha]|[op [i [k Ha]]]] ]]].
+      + eapply uPred.pure_soundness.
+        apply uPred.later_soundness in H.
+        iPoseProof H as "H".
+        iDestruct "H" as (β σ' en γ σ'' l' l'') "(H1 & H2 & H3)".
+        iExFalso.
+        iApply (internal_step_err σ e γ σ'' l').
+        iDestruct (internal_eq_rewrite α
+                     (Err e)
+                     (λ a, internal_step a σ γ σ'' l'%I) with "[] H2") as "H2'".
+        { solve_proper. }
+        { by iPureIntro. }
+        done.
+      + eapply uPred.pure_soundness.
+        apply uPred.later_soundness in H.
+        iPoseProof H as "H".
+        iDestruct "H" as (β σ' en γ σ'' l' l'') "(H1 & H2 & H3)".
+        iExFalso.
+        iApply (internal_step_ITV α (RetV n) γ σ σ'' l' with "[] H2").
+        iPureIntro.
+        rewrite Ha /=.
+        by rewrite IT_to_V_Ret.
+      + eapply uPred.pure_soundness.
+        apply uPred.later_soundness in H.
+        iPoseProof H as "H".
+        iDestruct "H" as (β σ' en γ σ'' l' l'') "(H1 & H2 & H3)".
+        iExFalso.
+        iApply (internal_step_ITV α (FunV g) γ σ σ'' l' with "[] H2").
+        iPureIntro.
+        rewrite Ha /=.
+        by rewrite IT_to_V_Fun.
+      + setoid_rewrite Ha.
+        assert (∃ (β : ITV) (σ' : stateO) (en : listO IT),
+                  external_steps r α' σ (IT_of_V β) σ' en m) as [β [σ' [en J]]].
+        {
+          apply IH.
+          iStartProof.
+          apply uPred.later_soundness in H.
+          iPoseProof H as "H".
+          iDestruct "H" as (β σ' en γ σ'' l' l'') "(H1 & H2 & H3)".
+          iDestruct (internal_eq_rewrite α
+                       (Tick α')
+                       (λ a, internal_step a σ γ σ'' l'%I) with "[] H2") as "H2'".
+          { solve_proper. }
+          { by iPureIntro. }
+          iClear "H2".
+          iRewrite "H1".
+          iClear "H1". clear H en.
+          iPoseProof (internal_step_tick with "H2'") as "(J1 & J2 & J3)".
+          iRewrite "J2". iRewrite "J3".
+          iRewrite "J3" in "H2'".
+          iClear "J3". clear l'.
+          iRewrite "J2" in "H2'".
+          iClear "J2".
+          clear σ.
+          iNext.
+          iRewrite - "J1".
+          iExists β, σ', l''.
+          iApply "H3".
+        }
+        {
+          exists β, σ', en.
+          eapply (steps_many r _ _ _ _ _ _ [] en en m); first done.
+          * apply external_step_tick; reflexivity.
+          * apply J.
+        }
+      + setoid_rewrite Ha.
+        destruct (reify r (Vis op i k) σ) as [[σ1 α1] en'] eqn:Hr.
+        assert ((∃ α1', α1 ≡ Tick α1') ∨ α1 ≡ Err RuntimeErr) as [[α1' Ha']|Ha'].
+        {
+          pose proof (reify_is_always_a_tick r op i k σ α1 σ1 en') as G.
+          apply G.
+          by rewrite Hr.
+        }
+        * cut (∃ (β : ITV) (σ' : stateO) (en : listO IT),
+                 external_steps r α1' σ1 (IT_of_V β) σ' en m).
+          {
+            intros [β [σ' [en J]]].
+            exists β, σ', (en' ++ en).
+            eapply (steps_many r _ _ _ _ _ _ en' en (en' ++ en)); first done.
+            - econstructor.
+              + reflexivity.
+              + rewrite Hr Ha'.
+                reflexivity.
+            - assumption.
+          }
+          {
+            apply IH.
+            apply uPred.later_soundness in H.
+            iPoseProof H as "H".
+            iDestruct "H" as (β σ' en γ σ'' l' l'') "(H1 & H2 & H3)".
+            iDestruct (internal_eq_rewrite α
+                         (Vis op i k)
+                         (λ a, internal_step a σ γ σ'' l'%I) with "[] H2") as "H2'".
+            { solve_proper. }
+            { by iPureIntro. }
+            iClear "H2".
+            iDestruct (internal_step_vis with "H2'") as "H2".
+            iClear "H2'".
+            rewrite Hr Ha'.
+            iDestruct (prod_equivI with "H2") as "(G1 & G2)".
+            iDestruct (prod_equivI with "G1") as "(G3 & G4)".
+            simpl.
+            iRewrite "G3".
+            iRewrite - "G2" in "H1".
+            iRewrite "H1".
+            iNext.
+            iRewrite "G4".
+            iExists β, σ', l''.
+            done.
+          }
+        * eapply uPred.pure_soundness.
+          apply uPred.later_soundness in H.
+          iPoseProof H as "H".
+          iDestruct "H" as (β σ' en γ σ'' l' l'') "(H1 & H2 & H3)".
+          iDestruct (internal_eq_rewrite α
+                       (Vis op i k)
+                       (λ a, internal_step a σ γ σ'' l'%I) with "[] H2") as "H2'".
+          { solve_proper. }
+          { by iPureIntro. }
+          iClear "H2".
+          iDestruct (internal_step_vis with "H2'") as "H2".
+          iClear "H2'".
+          rewrite Hr Ha'.
+          iExFalso.
+          iDestruct (prod_equivI with "H2") as "(G1 & _)".
+          iDestruct (prod_equivI with "G1") as "(_ & G4)".
+          simpl.
+          iApply IT_tick_err_ne. iApply internal_eq_sym. iAssumption.
+  Qed.
+
+  Lemma list_lookup_total_correct_I {X : ofe} `{!Inhabited X} (l : list X) (i : nat) (x : X) :
+    ⊢@{iProp} (l !! i ≡ Some x -∗ l !!! i ≡ x)%I.
+  Proof.
+    iIntros "H".
+    rewrite list_lookup_total_alt.
+    iRewrite "H".
+    done.
+  Qed.
+
+  Polymorphic Class FiniteExistential :=
+    can_split_or (P Q: nat → Prop):
+      (∀ a b, a < b → P b → P a) →
+      (∀ a b, a < b → Q b → Q a) →
+      (∀ a, P a ∨ Q a) → (∀ a, P a) ∨ (∀ a, Q a).
+
+  Polymorphic Class Classical : Prop :=
+    excluded_middle : ∀ P: Prop, P ∨ ¬ P.
+
+  Lemma classical_can_commute_or (P Q : nat → Prop):
+    (∀ P : Prop, P ∨ ¬ P) →
+    (∀ a b, a < b → P b → P a) →
+    (∀ a b, a < b → Q b → Q a) →
+    (∀ a, P a ∨ Q a) → (∀ a, P a) ∨ (∀ a, Q a).
+  Proof.
+    intros xm HdownP HdownQ Hsome.
+    destruct (xm (∃ a, ¬ P a)) as [[a' HP]|HP]; last first.
+    - left. intros a'. destruct (xm (P a')); auto.
+      exfalso. apply HP.
+      by exists a'.
+    - assert (Q a') by (destruct (Hsome a'); naive_solver).
+      right. intros b.
+      destruct (le_lt_dec a' b) as [J | J].
+      + destruct (le_lt_eq_dec _ _ J) as [K | K].
+        * destruct (Hsome b); auto.
+          exfalso.
+          apply HP.
+          eapply HdownP; eauto.
+        * by subst.
+      + eapply HdownQ; eauto.
+  Qed.
+
+  Global Instance classical_finite_existential `{Classical} : FiniteExistential.
+  Proof.
+    intros P Q ???. eapply classical_can_commute_or; eauto.
+  Qed.
+
+  Lemma can_commute_finite_exists `{FiniteExistential} (X : Type)
+    (P : X → nat → Prop) (Q: X → Prop) :
+    (∀ x a b, a < b → P x b → P x a)
+    → (∀ a, ∃ x, Q x ∧ P x a)
+    → pred_finite Q
+    → ∃ x, ∀ a, P x a.
+  Proof.
+    intros Hdown Hsome [Y Hfin].
+    assert (∀ a, ∃ x, x ∈ Y ∧ P x a) as Hsome'.
+    { intros a'. destruct (Hsome a') as [x [? ?]]. exists x. split; eauto. }
+    clear Hfin Hsome. induction Y as [|x Y IH].
+    - specialize (Hsome' 0) as [x [? ?]]. exfalso. by eapply not_elem_of_nil.
+    - assert ((∀ a, P x a) ∨ (∀ a : nat, ∃ x : X, x ∈ Y ∧ P x a)) as [|]; eauto.
+      eapply can_split_or; eauto.
+      + intros a' b Hab [y [HA HP]]. exists y; split; eauto.
+      + intros a'; destruct (Hsome' a') as [y [HA HP]].
+        apply elem_of_cons in HA as [<-|?]; eauto.
+  Qed.
+
+  Lemma iProp_disj `{Classical} (P Q : iProp)
+    : (⊢ P ∨ Q) → (⊢ P) ∨ ⊢ Q.
+  Proof.
+    intros J.
+    destruct (classical_can_commute_or (λ n, uPred_holds P n ε) (λ n, uPred_holds Q n ε)); eauto.
+    - intros b c Hbc K.
+      eapply uPred_mono; eauto. lia.
+    - intros b c Hbc K.
+      eapply uPred_mono; eauto. lia.
+    - intros n.
+      assert (Hemp : uPred_holds (emp : iProp) n ε).
+      { uPred.unseal. rewrite /upred.uPred_pure_def //=. }
+      pose proof (uPred_in_entails _ _ J n ε (ucmra_unit_validN _) Hemp) as G.
+      revert G.
+      uPred.unseal.
+      rewrite /= /upred.uPred_or_def /=.
+      intros [G | G]; by [left | right].
+    - left.
+      constructor.
+      intros n r' Hr Hval.
+      eapply uPred_mono; eauto.
+      apply ucmra_unit_leastN.
+    - right.
+      constructor.
+      intros n r' Hr Hval.
+      eapply uPred_mono; eauto.
+      apply ucmra_unit_leastN.
+  Qed.
+
+  Lemma iProp_finite_exists `{Classical}
+    X `{!EqDecision X} `{!finite.Finite X} (P : X → iProp)
+    : (⊢ ∃ a, P a) → ∃ a, ⊢ (P a).
+  Proof.
+    intros Hexist.
+    destruct (can_commute_finite_exists _
+                (λ a' n, uPred_holds (P a') n ε) (λ _, True)) as [x' H']; eauto.
+    - intros x b c Hbc J.
+      eapply uPred_mono; eauto. lia.
+    - intros n.
+      assert (Hemp : uPred_holds (emp : iProp) n ε).
+      { uPred.unseal. rewrite /upred.uPred_pure_def //=. }
+      pose proof (uPred_in_entails _ _ Hexist n ε (ucmra_unit_validN _) Hemp) as G.
+      revert G.
+      uPred.unseal.
+      rewrite /= /upred.uPred_exist_def /=.
+      intros [b G].
+      exists b.
+      split; first done.
+      apply G.
+    - exists (finite.enum X).
+      intros.
+      apply finite.elem_of_enum.
+    - exists x'.
+      constructor.
+      intros n x Hx Hval.
+      eapply uPred_mono; eauto.
+      apply ucmra_unit_leastN.
+  Qed.
+
+  Lemma tp_internal_steps_safe_agnostic `{C : Classical} α σ k :
+    (⊢ ∃ β βs σ', tp_internal_steps α σ ((IT_of_V β) :: βs) σ' k)
+    → (∃ β βs σ', tp_external_steps r α σ ((IT_of_V β) :: βs) σ' k).
+  Proof.
+    intros G.
+    assert (⊢ ▷ ∃ β βs σ', tp_internal_steps α σ ((IT_of_V β) :: βs) σ' k) as H.
+    {
+      iStartProof.
+      iPoseProof G as "H".
+      iNext. done.
+    }
+    clear G.
+    revert H.
+    revert α σ.
+    induction k as [| m IH]; intros α σ H.
+    - apply uPred.later_soundness in H.
+      setoid_rewrite tp_internal_steps_0 in H.
+      destruct α as [| α αs].
+      {
+        eapply uPred.pure_soundness.
+        iExFalso.
+        iPoseProof H as "H".
+        iDestruct "H" as (β βs σ') "(H1 & H2)".
+        iDestruct (list_equivI with "H1") as "J".
+        iSpecialize ("J" $! 0).
+        by iDestruct (option_equivI with "J") as "?".
+      }
+      destruct (IT_to_V α) as [β |] eqn:HEQ.
+      + exists β, αs, σ.
+        rewrite IT_of_to_V'; last by rewrite -HEQ.
+        by constructor.
+      + eapply uPred.pure_soundness.
+        iExFalso.
+        iPoseProof H as "H".
+        iDestruct "H" as (β βs σ') "(H1 & H2)".
+        iAssert (IT_to_V α ≡ IT_to_V (IT_of_V β))%I as "J".
+        {
+          iDestruct (list_equivI with "H1") as "J".
+          iSpecialize ("J" $! 0).
+          iSimpl in "J".
+          iDestruct (option_equivI with "J") as "?".
+          by iApply f_equivI.
+        }
+        rewrite IT_to_of_V.
+        rewrite HEQ.
+        by iDestruct (option_equivI with "J") as "?".
+    - setoid_rewrite tp_internal_steps_S in H.
+      cut (∃ (β : ITV) (βs : list IT) (σ' : stateO),
+             ∃ γ σ'', tp_external_step r α σ γ σ''
+                      ∧ tp_external_steps r γ σ'' (IT_of_V β :: βs) σ' m).
+      {
+        intros [β [βs [σ' [γ [σ'' [H1 H2]]]]]].
+        exists β, βs, σ'.
+        eapply tp_steps_many; eassumption.
+      }
+      rename H into H'.
+      assert (⊢ ▷ ∃ (x : list IT * list IT * IT),
+                    α ≡ x.1.1 ++ x.2 :: x.1.2
+                    ∧
+                      ∃ (σ'' : stateO) (δ' : IT) (en : list IT),
+                        internal_step x.2 σ δ' σ'' en
+                        ∧ ∃ (β : ITV) (βs : list IT) (σ' : stateO),
+                            tp_internal_steps (x.1.1 ++ δ' :: x.1.2 ++ en) σ''
+                              (IT_of_V β :: βs) σ' m) as H.
+      {
+        iStartProof.
+        iPoseProof H' as "H".
+        iNext.
+        iDestruct "H" as (β βs σ' γ σ'') "(H1 & H2)".
+        iDestruct "H1" as (α0 α1 δ δ' en) "(G1 & G2 & G3)".
+        iExists (α0, α1, δ).
+        iFrame "G1".
+        iExists σ''.
+        iExists δ', en.
+        iFrame "G3".
+        iExists β, βs, σ'.
+        iRewrite "G2" in "H2".
+        iFrame "H2".
+      }
+      clear H'.
+      cut (∃ (x : list IT * list IT * IT),
+             α ≡ x.1.1 ++ x.2 :: x.1.2
+             ∧ ∃ (σ'' : stateO) (δ' : IT) (en : list IT),
+                 (⊢ internal_step x.2 σ δ' σ'' en)
+                 ∧ ⊢ ∃ (β : ITV) (βs : list IT) (σ' : stateO),
+                     (tp_internal_steps (x.1.1 ++ δ' :: x.1.2 ++ en)
+                          σ'' (IT_of_V β :: βs) σ' m)).
+      {
+        intros [x [HEQ1 [σ'' [δ' [en [H1 H2]]]]]].
+        destruct x as [[α0 α1] δ].
+        edestruct IH as [β' [βs' [σ''' J1]]].
+        {
+          iNext.
+          iApply H2.
+        }
+        exists β', βs', σ''', (α0 ++ δ' :: α1 ++ en), σ''.
+        apply internal_step_safe in H1.
+        split; last done.
+        econstructor; last apply H1.
+        - apply HEQ1.
+        - reflexivity.
+      }
+      cut (∃ (x : list IT * list IT * IT),
+             α ≡ x.1.1 ++ x.2 :: x.1.2
+             ∧ ∃ (σ'' : stateO) (δ' : IT) (en : list IT),
+                 ⊢ (internal_step x.2 σ δ' σ'' en)
+                 ∧ ∃ (β : ITV) (βs : list IT) (σ' : stateO),
+                     (tp_internal_steps (x.1.1 ++ δ' :: x.1.2 ++ en)
+                        σ'' (IT_of_V β :: βs) σ' m)).
+      {
+        intros [x [HEQ1 [σ'' [δ' [en H1]]]]].
+        destruct x as [[α0 α1] δ].
+        exists (α0, α1, δ).
+        split; first done.
+        pose proof H1 as H2.
+        rewrite bi.and_elim_l in H2.
+        rewrite bi.and_elim_r in H1.
+        exists σ'', δ', en.
+        by split.
+      }
+      cut (∃ (x : list IT * list IT * IT),
+             α ≡ x.1.1 ++ x.2 :: x.1.2
+             ∧ ⊢ ∃ (σ'' : stateO) (δ' : IT) (en : list IT),
+                   (internal_step x.2 σ δ' σ'' en)
+                   ∧ ∃ (β : ITV) (βs : list IT) (σ' : stateO),
+                       (tp_internal_steps (x.1.1 ++ δ' :: x.1.2 ++ en)
+                          σ'' (IT_of_V β :: βs) σ' m)).
+      {
+        intros [x [HEQ1 H1]].
+        destruct x as [[α0 α1] δ].
+        exists (α0, α1, δ).
+        split; first done.
+        destruct (IT_dont_confuse δ)
+          as [[e Ha] | [[n Ha] | [ [g Ha] | [[α' Ha]|[op [i [k Ha]]]] ]]].
+        + eapply uPred.pure_soundness.
+          iExFalso.
+          iPoseProof H1 as "H".
+          iDestruct "H" as (σ'' δ' en) "(H1 & _)".
+          iApply (internal_step_err σ e δ' σ'' en).
+          iDestruct (internal_eq_rewrite δ
+                       (Err e)
+                       (λ a, internal_step a σ δ' σ'' en%I) with "[] H1") as "H1'".
+          { solve_proper. }
+          { by iPureIntro. }
+          done.
+        + eapply uPred.pure_soundness.
+          iExFalso.
+          iPoseProof H1 as "H".
+          iDestruct "H" as (σ'' δ' en) "(H1 & _)".
+          iExFalso.
+          iApply (internal_step_ITV δ (RetV n) δ' σ σ'' en with "[] H1").
+          iPureIntro.
+          rewrite Ha /=.
+          by rewrite IT_to_V_Ret.
+        + eapply uPred.pure_soundness.
+          iExFalso.
+          iPoseProof H1 as "H".
+          iDestruct "H" as (σ'' δ' en) "(H1 & _)".
+          iApply (internal_step_ITV δ (FunV g) δ' σ σ'' en with "[] H1").
+          iPureIntro.
+          rewrite Ha /=.
+          by rewrite IT_to_V_Fun.
+        + exists σ, α', [].
+          apply uPred.later_soundness.
+          iDestruct H1 as (σ'' δ' en) "(H1 & H2)".
+          iDestruct (internal_eq_rewrite δ
+                       (Tick α')
+                       (λ a, internal_step a σ δ' σ'' en%I) with "[] H1") as "H1'".
+          { solve_proper. }
+          { by iPureIntro. }
+          iPoseProof (internal_step_tick with "H1'") as "(J1 & J2 & J3)".
+          iNext.
+          iClear "H1'".
+          iRewrite "J1" in "H1".
+          iRewrite - "J2" in "H1".
+          iRewrite "J3" in "H1".
+          iFrame "H1".
+          iRewrite "J1" in "H2".
+          iRewrite - "J2" in "H2".
+          iRewrite "J3" in "H2".
+          iFrame "H2".
+        + destruct (reify r (Vis op i k) σ) as [[σ1 α1'] en'] eqn:Hr.
+          assert ((∃ α1'', α1' ≡ Tick α1'') ∨ α1' ≡ Err RuntimeErr)
+            as [[α1''' Ha']|Ha'].
+          {
+            pose proof (reify_is_always_a_tick r op i k σ α1' σ1 en') as G.
+            apply G.
+            by rewrite Hr.
+          }
+          * exists σ1, α1''', en'.
+            apply uPred.later_soundness.
+            iPoseProof H1 as "H".
+            iDestruct "H" as (σ'' δ' en) "(H1 & H2)".
+            iDestruct (internal_eq_rewrite δ
+                         (Vis op i k)
+                         (λ a, internal_step a σ δ' σ'' en%I) with "[] H1") as "H1'".
+            { solve_proper. }
+            { by iPureIntro. }
+            iDestruct (internal_step_vis with "H1'") as "H1''".
+            iDestruct (prod_equivI with "H1''") as "(G1 & G2)".
+            iDestruct (prod_equivI with "G1") as "(G3 & G4)".
+            rewrite Hr.
+            iSimpl in "G1 G2 G3 G4".
+            iRewrite - "G2" in "H1".
+            iRewrite - "G3" in "H1".
+            iEval (rewrite Ha') in "G4".
+            iNext.
+            iRewrite - "G4" in "H1".
+            iFrame "H1".
+            iRewrite - "G2" in "H2".
+            iRewrite - "G3" in "H2".
+            iRewrite - "G4" in "H2".
+            iFrame "H2".
+          * eapply uPred.pure_soundness.
+            iPoseProof H1 as "H".
+            iDestruct "H" as (σ'' δ' en) "(H1 & H2)".
+            iDestruct (internal_eq_rewrite δ
+                         (Vis op i k)
+                         (λ a, internal_step a σ δ' σ'' en%I) with "[] H1") as "H1'".
+            { solve_proper. }
+            { by iPureIntro. }
+            iDestruct (internal_step_vis with "H1'") as "H1''".
+            rewrite Hr Ha'.
+            iExFalso.
+            iDestruct (prod_equivI with "H1''") as "(G1 & _)".
+            iDestruct (prod_equivI with "G1") as "(_ & G4)".
+            simpl.
+            iApply IT_tick_err_ne. iApply internal_eq_sym. iAssumption.
+      }
+      apply uPred.later_soundness in H.
+      clear IH.
+      cut (∃ i : fin (length α),
+             ⊢ ∃ (σ'' : stateO) (δ' : IT) (en : list IT),
+                 internal_step (Vector.of_list α !!! i) σ δ' σ'' en
+                 ∧ ∃ (β : ITV) (βs : list IT) (σ' : stateO),
+                     tp_internal_steps
+                       (take i (list_to_vec α) ++ δ' :: drop (S i) (list_to_vec α)
+                          ++ en) σ''
+                       (IT_of_V β :: βs) σ' m).
+      {
+        intros [i G].
+        exists (take i (list_to_vec α), drop (S i) (list_to_vec α), (Vector.of_list α !!! i)).
+        split.
+        - rewrite /=; rewrite -vec_to_list_take_drop_lookup.
+          by rewrite vec_to_list_to_vec.
+        - iApply G.
+      }
+      assert (⊢ ∃ i : fin (length α),
+                ∃ (σ'' : stateO) (δ' : IT) (en : list IT),
+                  internal_step (Vector.of_list α !!! i) σ δ' σ'' en
+                  ∧ ∃ (β : ITV) (βs : list IT) (σ' : stateO),
+                      tp_internal_steps
+                        (take i (list_to_vec α) ++ δ' :: drop (S i) (list_to_vec α)
+                           ++ en) σ''
+                        (IT_of_V β :: βs) σ' m).
+      {
+        iPoseProof H as "H".
+        iDestruct "H" as (x) "(H1 & H2)".
+        destruct x as [[x1 x2] x3].
+        rewrite vec_to_list_to_vec.
+        iAssert (⌜∃ i : fin (length α), (i : nat) = length x1⌝)%I as "%J".
+        {
+          iAssert (⌜length x1 < length α⌝)%I as "%J".
+          {
+            iDestruct (f_equivI length with "H1") as "%J".
+            iPureIntro.
+            rewrite /= length_app length_cons in J.
+            symmetry in J.
+            lia.
+          }
+          iExists (nat_to_fin J).
+          iPureIntro.
+          by rewrite fin_to_nat_to_fin.
+        }
+        destruct J as [i J].
+        iExists i.
+        iAssert (x3 ≡ list_to_vec α !!! i)%I as "HEQ1".
+        {
+          iDestruct (list_equivI with "H1") as "H1'".
+          iSpecialize ("H1'" $! i).
+          iSimpl in "H1 H1'".
+          rewrite list_lookup_middle; last done.
+          iApply internal_eq_sym.
+          iClear "H1 H2".
+          clear.
+          iPoseProof (list_lookup_total_correct_I (X := IT) (list_to_vec α) i x3 with "[]") as "J".
+          - iRewrite - "H1'".
+            iPureIntro.
+            by rewrite vec_to_list_to_vec.
+          - iRewrite - "J".
+            iPureIntro.
+            match goal with
+            | |- context G [?a ≡ ?b] =>
+                assert (a = b) as ->; last done
+            end.
+            rewrite vec_to_list_to_vec.
+            rewrite vlookup_lookup.
+            rewrite vec_to_list_to_vec.
+            apply list_lookup_lookup_total_lt.
+            apply fin_to_nat_lt.
+        }
+        iDestruct "H2" as (σ'' δ' en) "(J1 & J2)".
+        iExists σ'', δ', en.
+        iSplit.
+        { by iRewrite "HEQ1" in "J1". }
+        iDestruct "J2" as (β βs σ') "J2".
+        iExists β, βs, σ'.
+        iSimpl in "J2".
+        iAssert ((take i α ++ δ' :: drop (S i) α ++ en) ≡
+                   (x1 ++ δ' :: x2 ++ en))%I as "HEQ2".
+        {
+          iApply list_equivI.
+          iIntros (n).
+          destruct (lt_eq_lt_dec n i) as [[K | ->] | K].
+          - rewrite lookup_app_l.
+            + iDestruct (list_equivI with "H1") as "H1'".
+              iSpecialize ("H1'" $! n).
+              iSimpl in "H1'".
+              rewrite lookup_take; last done.
+              iRewrite "H1'".
+              rewrite lookup_app_l; last (by rewrite -J).
+              rewrite lookup_app_l; first done; last (by rewrite -J).
+            + rewrite firstn_length_le; first done.
+              apply Nat.lt_le_incl.
+              apply fin_to_nat_lt.
+          - rewrite J.
+            rewrite list_lookup_middle.
+            + by rewrite list_lookup_middle.
+            + rewrite length_take_le; first done.
+              rewrite -J.
+              apply Nat.lt_le_incl.
+              apply fin_to_nat_lt.
+          - rewrite lookup_app_r.
+            + iDestruct (list_equivI with "H1") as "H1'".
+              iSpecialize ("H1'" $! n).
+              iSimpl in "H1'".
+              rewrite length_take_le; last (apply Nat.lt_le_incl, fin_to_nat_lt).
+              rewrite lookup_app_r; last (rewrite -J; by apply Nat.lt_le_incl).
+              rewrite lookup_app_r; last (rewrite -J; by apply Nat.lt_le_incl).
+              rewrite -J.
+              rewrite lookup_cons_ne_0; last lia.
+              rewrite lookup_cons_ne_0; last lia.
+              rewrite lookup_cons_ne_0; last lia.
+              destruct (decide (n < length α)) as [L | L].
+              * rewrite lookup_app_l.
+                -- rewrite lookup_drop.
+                   rewrite Nat.add_pred_r; last lia.
+                   rewrite Nat.add_succ_l.
+                   rewrite Nat.add_sub_assoc; last lia.
+                   rewrite Nat.add_sub' /=.
+                   iAssert (⌜Init.Nat.pred (n - i) < length x2⌝)%I as "%J'".
+                   {
+                     iDestruct (f_equivI length with "H1") as "%J'".
+                     iPureIntro.
+                     rewrite /= length_app length_cons -J in J'.
+                     lia.
+                   }
+                   iRewrite "H1'".
+                   by rewrite lookup_app_l.
+                -- rewrite length_drop.
+                   rewrite Nat.sub_succ_r.
+                   rewrite -Nat.pred_lt_mono; last lia.
+                   lia.
+              * rewrite lookup_app_r.
+                -- iAssert (⌜length x2 <= Init.Nat.pred (n - i)⌝)%I as "%J'".
+                   {
+                     iDestruct (f_equivI length with "H1") as "%J'".
+                     iPureIntro.
+                     rewrite /= length_app length_cons -J in J'.
+                     lia.
+                   }
+                   rewrite lookup_app_r; last done.
+                   iAssert (⌜length (drop (S i) α) = length x2⌝)%I as "%J''".
+                   {
+                     rewrite length_drop.
+                     iDestruct (f_equivI length with "H1") as "%J''".
+                     iPureIntro.
+                     rewrite /= length_app length_cons -J in J''.
+                     lia.
+                   }
+                   by rewrite J''.
+                -- rewrite length_drop.
+                   rewrite Nat.sub_succ_r.
+                   lia.
+            + rewrite length_take_le; first lia.
+              apply Nat.lt_le_incl.
+              apply fin_to_nat_lt.
+        }
+        by iRewrite "HEQ2".
+      }
+      eapply iProp_finite_exists.
+      + apply _.
+      + assumption.
   Qed.
 
 End internal_step.
