theories/gitree/logrel.v
@@ -1,0 +1,1741 @@
+From iris.algebra Require Import excl auth frac agree gmap list gmap_view.
+From iris.algebra.lib Require Import excl_auth.
+From iris.proofmode Require Import base tactics classes modality_instances.
+From iris.base_logic.lib Require Export own fancy_updates invariants mono_nat.
+From gitrees Require Import prelude.
+From gitrees.gitree Require Import core reify greifiers reductions weakestpre lambda.
+From gitrees Require Import hom.
+
+Definition specN := nroot .@ "spec".
+Definition stateN := nroot .@ "state".
+
+Lemma take_drop_middle_L :
+  ∀ {A : ofe} (l : list A) (i : nat) (x : A),
+  l !! i ≡ Some x → take i l ++ x :: drop (S i) l ≡ l.
+Proof.
+  intros A l.
+  induction l as [| x l Hl].
+  - intros ?? H; simpl.
+    exfalso.
+    rewrite lookup_nil in H.
+    inversion H.
+  - intros i y H.
+    simpl.
+    destruct i as [| i].
+    + simpl.
+      rewrite drop_0.
+      simpl in H.
+      inversion H; subst.
+      f_equiv; by symmetry.
+    + simpl.
+      f_equiv.
+      simpl in H.
+      by apply (Hl i y).
+Qed.
+
+Lemma lookup_lt_Some_L : ∀ {A : ofe} (l : list A) (i : nat) (x : A),
+  l !! i ≡ Some x → i < length l.
+Proof.
+  intros ? l.
+  induction l as [| y l Hl]; intros G.
+  - intros ? J; inversion J.
+  - intros x J.
+    simpl.
+    destruct G as [| G].
+    + simpl in J.
+      lia.
+    + rewrite -Nat.succ_lt_mono.
+      eapply Hl.
+      apply J.
+Qed.
+
+Lemma lookup_geq_None_L : ∀ {A : ofe} (l : list A) (i : nat),
+  l !! i ≡ None → i ≥ length l.
+Proof.
+  intros ? l.
+  induction l as [| y l Hl]; intros G.
+  - intros J; inversion J.
+    simpl.
+    lia.
+  - intros J.
+    simpl.
+    destruct G as [| G].
+    + simpl in J.
+      inversion J.
+    + simpl in J.
+      apply Hl in J.
+      lia.
+Qed.
+
+Lemma lookup_geq_None_L_inv : ∀ {A : ofe} (l : list A) (i : nat),
+  i ≥ length l → l !! i = None.
+Proof.
+  intros ? l.
+  induction l as [| y l Hl]; intros G.
+  - intros J.
+    done.
+  - intros J.
+    simpl in J.
+    assert (∃ G', G = S G') as [G' ->].
+    {
+      inversion J as [ | J'].
+      - exists (length l).
+        lia.
+      - exists J'.
+        lia.
+    }
+    simpl.
+    apply Hl.
+    lia.
+Qed.
+
+Lemma tp_external_steps_many_L {a} {rs : sReifier a} `{!Cofe A}
+  (α1 : listO (IT (sReifier_ops rs) A)) σ1 α2 σ2 α3 σ3 n2 :
+  tp_external_step rs α2 σ2 α3 σ3 →
+  tp_external_steps rs α1 σ1 α2 σ2 n2 →
+  tp_external_steps rs α1 σ1 α3 σ3 (S n2).
+Proof.
+  intros G H; revert G.
+  induction H as [| ????????? IH]; intros G.
+  - setoid_subst.
+    econstructor; last constructor; first apply G; done.
+  - by econstructor; last by apply IH; done.
+Qed.
+
+Lemma tp_internal_steps_many_L {a} {rs : sReifier a} `{!Cofe A}
+  {Σ}
+  (α1 : listO (IT (sReifier_ops rs) A)) σ1 α2 σ2 α3 σ3 n2 :
+  ⊢ tp_internal_step (Σ := Σ) rs α2 σ2 α3 σ3
+    -∗ tp_internal_steps rs α1 σ1 α2 σ2 n2
+    -∗ tp_internal_steps rs α1 σ1 α3 σ3 (S n2).
+Proof.
+  iRevert (α1 σ1 α2 σ2 α3 σ3).
+  iInduction n2 as [| n2 IH] "IH";
+    iIntros (α1 σ1 α2 σ2 α3 σ3).
+  - iIntros "G H".
+    rewrite tp_internal_steps_0.
+    iDestruct "H" as "(H1 & H2)".
+    iRewrite "H1". iRewrite "H2".
+    rewrite tp_internal_steps_S.
+    iExists α3, σ3.
+    iSplit; first done.
+    by rewrite tp_internal_steps_0.
+  - iIntros "G H".
+    iEval (rewrite tp_internal_steps_S) in "H".
+    iDestruct "H" as "(%γ & %σ' & H1 & H2)".
+    iPoseProof ("IH" $! γ σ' α2 σ2 α3 σ3 with "G H2") as "J".
+    iEval (rewrite tp_internal_steps_S).
+    iExists γ, σ'.
+    by iSplit.
+Qed.
+
+Lemma IT_tau_err_ne' `{Cofe R} {F} α e :
+  (Tau (A := R) (E := F) α ≡ Err e → False).
+Proof.
+  intros H1.
+  assert (IT_unfold (Tau α) ≡ IT_unfold (Err e)) as H2.
+  { by rewrite H1. }
+  rewrite !IT_unfold_fold /= in H2.
+  inversion H2 as [?? G |]; subst.
+  inversion G.
+Qed.
+
+Transparent Tau.
+Lemma Tau_inj'' `{Cofe R} {F} (α β : laterO (IT F R)) :
+  ((Tau α ≡ Tau β) → α ≡ β).
+Proof.
+  intros T.
+  assert ((IT_unfold (Tau α)) ≡ (IT_unfold (Tau β))) as G.
+  { rewrite T. done. }
+  unfold Tau in G. simpl in G.
+  rewrite !IT_unfold_fold in G.
+  inversion G as [?? J |]; subst.
+  inversion J; subst.
+  done.
+Qed.
+Opaque Tau.
+
+Lemma reify_vis_cont {rs : sReifier NotCtxDep} `{!Cofe R}
+  op i k1 k2 σ1 σ2 β th :
+  (reify (A := R) rs (Vis op i k1) σ1 ≡
+     (σ2, Tick β, th) →
+   reify rs (Vis op i (laterO_map k2 ◎ k1)) σ1 ≡
+     (σ2, Tick (k2 β), th)).
+Proof.
+  destruct (sReifier_re rs op (i,σ1))
+    as [[[o σ2'] th']|] eqn:Hre; last first.
+  - rewrite reify_vis_None_ctx_indep; last by rewrite Hre//.
+    intros Hr.
+    exfalso.
+    destruct Hr as [[_ Hr2] _].
+    simpl in Hr2.
+    symmetry in Hr2.
+    by apply IT_tau_err_ne' in Hr2.
+  - rewrite reify_vis_eq_ctx_indep; last first.
+    { by rewrite Hre. }
+    rewrite reify_vis_eq_ctx_indep; last first.
+    { by rewrite Hre. }
+    intros Hr.
+    destruct Hr as [[Hr1 Hr2] Hr3].
+    simpl in *.
+    rewrite Tick_eq in Hr2.
+    rewrite Hr1.
+    rewrite -Hr3.
+    do 2 f_equiv.
+    apply Tau_inj'' in Hr2.
+    rewrite Hr2.
+    rewrite later_map_Next.
+    reflexivity.
+Qed.
+
+Lemma external_step_ectx {rs : sReifier NotCtxDep} `{!Cofe A}
+  (K : HOM) (e : IT (sReifier_ops rs) A) e' σ σ' efs :
+  external_step rs e σ e' σ' efs
+  → external_step rs (K e) σ (K e') σ' efs.
+Proof.
+  intros H.
+  destruct H as [???? H1 H2 | ???????? H1 H2].
+  - rewrite H1 H2.
+    rewrite hom_tick.
+    by constructor.
+  - rewrite H1.
+    rewrite hom_vis.
+    econstructor.
+    + reflexivity.
+    + assert (reify rs (Vis op i k) σ1 ≡ (σ2, Tick β, th))
+        as J.
+      {
+        rewrite -H2.
+        do 2 f_equiv.
+        symmetry.
+        done.
+      }
+      pose proof (reify_vis_cont op i k (λne x, K x) σ1 σ2 β th J) as L.
+      simpl in J.
+      rewrite -L.
+      do 3 f_equiv.
+      intros ?.
+      reflexivity.
+Qed.
+
+Lemma external_step_ectx' {n} {rs : gReifiers NotCtxDep n} `{!Cofe A}
+  (K : HOM) (e : IT (gReifiers_ops rs) A) e' σ σ' efs :
+  external_step (gReifiers_sReifier rs) e σ e' σ' efs
+  → external_step (gReifiers_sReifier rs) (K e) σ (K e') σ' efs.
+Proof.
+  intros H.
+  destruct H as [???? H1 H2 | ???????? H1 H2].
+  - rewrite H1 H2.
+    rewrite hom_tick.
+    by constructor.
+  - rewrite H1.
+    rewrite hom_vis.
+    econstructor.
+    + reflexivity.
+    + assert (reify _ (Vis op i k) σ1 ≡ (σ2, Tick β, th))
+        as J.
+      {
+        rewrite -H2.
+        do 2 f_equiv.
+        symmetry.
+        done.
+      }
+      pose proof (reify_vis_cont op i k (λne x, K x) σ1 σ2 β th J) as L.
+      simpl in J.
+      rewrite -L.
+      do 3 f_equiv.
+      intros ?.
+      reflexivity.
+Qed.
+
+Lemma tp_internal_steps_trans
+  {a} {rs : sReifier a} `{!Cofe A} {Σ}
+  (α1 : listO (IT (sReifier_ops rs) A)) σ1 α2 σ2 α3 σ3 n2 m2 :
+  ⊢ tp_internal_steps (Σ := Σ) rs α2 σ2 α3 σ3 m2
+    -∗ tp_internal_steps rs α1 σ1 α2 σ2 n2
+    -∗ tp_internal_steps rs α1 σ1 α3 σ3 (m2 + n2).
+Proof.
+  iRevert (α1 σ1 α2 σ2 α3 σ3 n2).
+  iInduction m2 as [| m2 IH] "IH";
+    iIntros (α1 σ1 α2 σ2 α3 σ3 n2).
+  - iIntros "G H".
+    rewrite tp_internal_steps_0.
+    iDestruct "G" as "(G1 & G2)".
+    iRewrite - "G1". iRewrite - "G2".
+    rewrite Nat.add_0_l.
+    done.
+  - iIntros "G H".
+    iEval (rewrite tp_internal_steps_S) in "G".
+    iDestruct "G" as "(%γ & %σ' & G1 & G2)".
+    rewrite Nat.add_succ_l -Nat.add_succ_r.
+    iDestruct (tp_internal_steps_many_L with "G1 H") as "K".
+    iApply ("IH" with "G2 K").
+Qed.
+
+Lemma tp_internal_steps_trans'
+  {n} {rs : gReifiers NotCtxDep n} `{!Cofe A} {Σ}
+  (α1 : listO (IT (gReifiers_ops rs) A)) σ1 α2 σ2 α3 σ3 n2 m2 :
+  ⊢ tp_internal_steps (Σ := Σ) (gReifiers_sReifier rs) α2 σ2 α3 σ3 m2
+    -∗ tp_internal_steps (gReifiers_sReifier rs) α1 σ1 α2 σ2 n2
+    -∗ tp_internal_steps (gReifiers_sReifier rs) α1 σ1 α3 σ3 (m2 + n2).
+Proof.
+  iRevert (α1 σ1 α2 σ2 α3 σ3 n2).
+  iInduction m2 as [| m2 IH] "IH";
+    iIntros (α1 σ1 α2 σ2 α3 σ3 n2).
+  - iIntros "G H".
+    rewrite tp_internal_steps_0.
+    iDestruct "G" as "(G1 & G2)".
+    iRewrite - "G1". iRewrite - "G2".
+    rewrite Nat.add_0_l.
+    done.
+  - iIntros "G H".
+    iEval (rewrite tp_internal_steps_S) in "G".
+    iDestruct "G" as "(%γ & %σ' & G1 & G2)".
+    rewrite Nat.add_succ_l -Nat.add_succ_r.
+    iDestruct (tp_internal_steps_many_L with "G1 H") as "K".
+    iApply ("IH" with "G2 K").
+Qed.
+
+Class monoSG Σ := MONOSG { mono_inG :: mono_natG Σ; mono_name : gname }.
+
+Section steps.
+  Context `{!monoSG Σ}.
+
+  Local Definition steps_auth (n : nat) : iProp Σ :=
+    mono_nat_auth_own mono_name 1 n.
+
+  Definition steps_lb (n : nat) : iProp Σ :=
+    mono_nat_lb_own mono_name n.
+
+  Lemma steps_lb_0 :
+    ⊢ |==> steps_lb 0.
+  Proof. by apply mono_nat_lb_own_0. Qed.
+
+  Local Lemma steps_lb_valid n m :
+    steps_auth n -∗ steps_lb m -∗ ⌜m ≤ n⌝.
+  Proof.
+    iIntros "Hauth Hlb".
+    by iDestruct (mono_nat_lb_own_valid with "Hauth Hlb") as %[_ Hle].
+  Qed.
+
+  Local Lemma steps_lb_get n :
+    steps_auth n -∗ steps_lb n.
+  Proof. apply mono_nat_lb_own_get. Qed.
+
+  Local Lemma steps_auth_update n n' :
+    n ≤ n' → steps_auth n ==∗ steps_auth n' ∗ steps_lb n'.
+  Proof. intros Hle. by apply mono_nat_own_update. Qed.
+
+  Local Lemma steps_auth_update_S n :
+    steps_auth n ==∗ steps_auth (S n).
+  Proof.
+    iIntros "Hauth".
+    iMod (mono_nat_own_update with "Hauth") as "[$ _]"; [lia|done].
+  Qed.
+
+  Lemma steps_lb_le n n' :
+    n' ≤ n → steps_lb n -∗ steps_lb n'.
+  Proof. intros Hle. by iApply mono_nat_lb_own_le. Qed.
+
+End steps.
+
+Section tp.
+  Context {n : nat} {a : is_ctx_dep} (rs : gReifiers a n).
+  Notation F := (gReifiers_ops rs).
+  Context (R : ofe) `{!Cofe R}.
+  Notation IT := (IT F R).
+  Notation ITV := (ITV F R).
+
+  Definition tpoolUR : ucmra := gmap_viewR nat (agreeR IT).
+
+  Fixpoint to_tpool_go (i : nat) (tp : listO IT) : gmap nat (agreeR IT) :=
+    match tp with
+    | [] => ∅
+    | e :: tp => <[i:=to_agree e]>(to_tpool_go (S i) tp)
+    end.
+
+  Lemma to_tpool_go_lookup (tp : listO IT) i :
+    ∀ k j, to_tpool_go k tp !! j = to_tpool_go (k + i) tp !! (j + i).
+  Proof.
+    revert i.
+    induction tp as [| ? tp IH].
+    - done.
+    - simpl.
+      intros i k j.
+      destruct (decide (k = j)); [subst |].
+      + by rewrite !lookup_insert.
+      + rewrite lookup_insert_ne; last done.
+        rewrite (IH i (S k) j) /=.
+        rewrite lookup_insert_ne; last lia.
+        reflexivity.
+  Qed.
+
+  Lemma to_tpool_go_lookup' (tp : listO IT) :
+    ∀ j k, to_agree <$> tp !! j = to_tpool_go k tp !! (k + j).
+  Proof.
+    induction tp as [| x tp IH].
+    - intros ?; simpl.
+      done.
+    - intros j; simpl.
+      destruct j as [| j].
+      + simpl.
+        intros k.
+        rewrite Nat.add_0_r.
+        destruct (decide (k = 0)); [subst |].
+        * by rewrite lookup_insert.
+        * by rewrite lookup_insert.
+      + simpl.
+        intros k.
+        rewrite lookup_insert_ne; last lia.
+        rewrite -Nat.add_succ_comm.
+        rewrite -IH.
+        reflexivity.
+  Qed.
+
+  Lemma to_tpool_go_comm_insert (tp : listO IT) j (H : j < length tp) x :
+    to_tpool_go 0 (<[j := x]> tp) = <[j := to_agree x]> (to_tpool_go 0 tp).
+  Proof.
+    apply map_eq.
+    intros q.
+    rewrite -!(to_tpool_go_lookup' _ _ 0).
+    destruct (decide (j = q)); [subst |].
+    - rewrite lookup_insert.
+      by rewrite list_lookup_insert; last done.
+    - rewrite list_lookup_insert_ne; last done.
+      rewrite lookup_insert_ne; last done.
+      by rewrite (to_tpool_go_lookup' _ _ 0).
+  Qed.
+
+  Lemma to_tpool_go_comm_union (tp tp' : listO IT) :
+    ∀ k, to_tpool_go k (tp ++ tp') = (to_tpool_go k tp) ∪ (to_tpool_go (k + length tp) tp').
+  Proof.
+    revert tp'.
+    induction tp as [| ? ? IH].
+    - intros; simpl.
+      symmetry.
+      rewrite Nat.add_0_r.
+      apply (map_empty_union (to_tpool_go k tp')).
+    - intros tp' k.
+      rewrite /= IH Nat.add_succ_comm.
+      by rewrite insert_union_l.
+  Qed.
+
+  Lemma to_tpool_go_map_to_list (tp : listO IT) :
+    ∀ k, (map_to_list (to_tpool_go k tp)) ≡ₚ (zip (seq k (length tp)) (to_agree <$> tp)).
+  Proof.
+    induction tp as [| ? ? IH].
+    - done.
+    - intros k.
+      rewrite /= -IH.
+      rewrite map_to_list_insert; first done.
+      replace (S k) with (1 + k) by reflexivity.
+      assert (1 + k > k) as H; first lia.
+      revert H.
+      generalize (1 + k).
+      generalize k.
+      clear.
+      induction tp as [| ? ? IH]; intros k p H.
+      + done.
+      + intros.
+        rewrite /= lookup_insert_ne; last lia.
+        apply IH; lia.
+  Qed.
+
+  Program Definition to_tpool' : listO IT -> tpoolUR := λ l, ●V (to_tpool_go 0 l).
+
+  Program Definition to_tpool : listO IT -n> tpoolUR := λne l, (to_tpool' l).
+  Next Obligation.
+    rewrite /to_tpool'.
+    intros p l.
+    generalize 0.
+    induction l as [| x l Hl]; intros m ? H.
+    - apply Forall2_nil_inv_l in H.
+      rewrite H.
+      reflexivity.
+    - apply Forall2_cons_inv_l in H.
+      destruct H as [x' [l' [H1 [H2 H3]]]].
+      rewrite H3.
+      simpl.
+      do 2 f_equiv.
+      + solve_proper.
+      + specialize (Hl (S m) l' H2).
+        destruct Hl as [Hl _].
+        simpl in Hl.
+        apply Some_dist_inj in Hl.
+        apply pair_dist_inj in Hl.
+        destruct Hl as [_ Hl].
+        apply to_agree_injN in Hl.
+        apply Hl.
+  Qed.
+
+  Class tpoolSG Σ := TPOOLSG { tpool_inG :: inG Σ ( tpoolUR); tpool_name : gname }.
+End tp.
+
+Section right_hand_side.
+  Context {n : nat} (rs : gReifiers NotCtxDep n).
+  Notation F := (gReifiers_ops rs).
+  Context (R : ofe) `{!Cofe R}.
+  Notation IT := (IT F R).
+  Notation ITV := (ITV F R).
+  Context {Σ : gFunctors}.
+  Context `(HSTATE : !stateG rs R Σ).
+  Context `{!invGS_gen HasLc Σ} `{!tpoolSG rs R Σ}.
+  Notation iProp := (iProp Σ).
+  Notation coPsetO := (leibnizO coPset).
+  Context (s : stuckness).
+  Notation HOM := (@HOM R _ F).
+
+  Program Definition tpool_pointsto (j : natO) (e : IT) : iProp :=
+    own (tpool_name rs R) (gmap_view_frag j (DfracOwn 1) (to_agree e)).
+
+  Global Instance tpool_pointsto_ne l : NonExpansive (tpool_pointsto l).
+  Proof.
+    intros ??? H.
+    rewrite /tpool_pointsto.
+    do 3 f_equiv.
+    done.
+  Qed.
+
+  Global Instance tpool_pointsto_proper l : Proper ((≡) ==> (≡)) (tpool_pointsto l).
+  Proof.
+    intros ?? H.
+    rewrite /tpool_pointsto.
+    do 3 f_equiv.
+    apply H.
+  Qed.
+
+  Notation "j ⤇ e" := (tpool_pointsto j e) (at level 20) : bi_scope.
+
+  Program Definition spec_inv (ρ : listO IT) σ : iProp :=
+    (∃ tp σ' m, own (tpool_name rs R) ((to_tpool rs R tp))
+                ∗ @state_interp _ _ _ _ _ _ HSTATE σ'
+                ∗ tp_internal_steps (gReifiers_sReifier rs) ρ σ tp σ' m)%I.
+
+  Definition spec_ctx : iProp :=
+    (∃ ρ σ, inv specN (spec_inv ρ σ))%I.
+
+  Global Instance spec_ctx_persistent : Persistent spec_ctx.
+  Proof. apply _. Qed.
+
+  Lemma step_insert (K : HOM) (tp : listO IT) j e σ e' σ' efs :
+    tp !! j ≡ Some (K e) → external_step (gReifiers_sReifier rs) e σ e' σ' efs →
+    tp_external_step (gReifiers_sReifier rs) tp σ (<[j:=K e']> tp ++ efs) σ'.
+  Proof.
+    intros.
+    rewrite -(take_drop_middle_L tp j (K e)) //.
+    rewrite insert_app_r_alt; first last.
+    {
+      rewrite length_take_le; first reflexivity.
+      apply Nat.lt_le_incl.
+      eapply lookup_lt_Some_L; eassumption.
+    }
+    econstructor.
+    - reflexivity.
+    - rewrite -assoc_L.
+      f_equiv.
+      rewrite length_take_le; first last.
+      {
+        apply Nat.lt_le_incl.
+        eapply lookup_lt_Some_L.
+        eassumption.
+      }
+      rewrite Nat.sub_diag.
+      simpl.
+      reflexivity.
+    -
+      by apply external_step_ectx'.
+  Qed.
+
+  Lemma step_insert_no_fork (K : HOM) (tp : listO IT) j e σ e' σ' :
+    tp !! j ≡ Some (K e) → external_step (gReifiers_sReifier rs) e σ e' σ' [] →
+    tp_external_step (gReifiers_sReifier rs) tp σ (<[j:=K e']> tp) σ'.
+  Proof. rewrite -(right_id_L [] (++) (<[_:=_]>_)). by apply step_insert. Qed.
+
+  Lemma tpool_read l α tp :
+    own (tpool_name rs R) (to_tpool rs R tp)
+    -∗ tpool_pointsto l α
+    -∗ (tp !! l) ≡ Some α.
+  Proof.
+    iIntros "Ha Hf".
+    iPoseProof (own_valid_2 with "Ha Hf") as "H".
+    rewrite gmap_view_both_validI.
+    iDestruct "H" as "[%H Hval]".
+    rewrite option_equivI.
+    rewrite -(to_tpool_go_lookup' rs R tp l 0).
+    destruct (tp !! l) as [o |] eqn:Heq.
+    - rewrite Heq /=.
+      rewrite agree_equivI.
+      iDestruct "Hval" as "(_ & Hval)".
+      by iRewrite "Hval".
+    - rewrite Heq /=.
+      iDestruct "Hval" as "(_ & Hval)".
+      done.
+  Qed.
+
+  Lemma tpool_alloc α l σ :
+    σ !! l = None →
+    own (tpool_name rs R) (to_tpool rs R σ)
+    ==∗ own (tpool_name rs R) (●V (<[l:=to_agree (α)]>(to_tpool_go rs R 0 σ)))
+                   ∗ tpool_pointsto l α.
+  Proof.
+    iIntros (Hl) "H".
+    iMod (own_update with "H") as "[$ $]".
+    { apply (gmap_view_alloc _ l (DfracOwn 1) (to_agree (α))); eauto.
+      - rewrite -(to_tpool_go_lookup' rs R σ l 0).
+        by rewrite Hl.
+      - done.
+      - done.
+    }
+    done.
+  Qed.
+
+  Lemma tpool_alloc_big (α : listO IT) σ :
+    own (tpool_name rs R) (to_tpool rs R σ)
+    ==∗ own (tpool_name rs R)
+          (●V ((to_tpool_go rs R 0 σ) ∪ (to_tpool_go rs R (length σ) α)))
+                   ∗ [∗ list] i ∈ α, ∃ j, tpool_pointsto j i.
+  Proof.
+    iIntros "H".
+    assert (∀ k, to_tpool_go rs R (k + (length σ)) α ##ₘ to_tpool_go rs R k σ) as HD.
+    {
+      induction σ as [| x σ IH].
+      - intros; apply map_disjoint_empty_r.
+      - intros k; simpl.
+        apply map_disjoint_insert_r_2.
+        + rewrite Nat.add_comm.
+          rewrite -(to_tpool_go_lookup rs R α k (S (length σ)) 0).
+          clear.
+          generalize (length σ).
+          induction α as [| ? ? IH].
+          * done.
+          * intros m; simpl.
+            rewrite lookup_insert_ne; last done.
+            apply IH.
+        + rewrite -Nat.add_1_l Nat.add_assoc (Nat.add_comm k).
+          apply IH.
+    }
+    iMod (own_update with "H") as "[H1 H2]".
+    {
+      specialize (HD 0).
+      simpl in HD.
+      apply (gmap_view_alloc_big (to_tpool_go rs R 0 σ)
+                     (to_tpool_go rs R (length σ) α)
+                     (DfracOwn 1) HD); eauto.
+      - done.
+      - apply map_Forall_lookup_2.
+        intros i x H.
+        admit.
+    }
+    rewrite map_union_comm; last apply (HD 0).
+    iModIntro.
+    iSplitL "H1".
+    - unfold gmap_view_auth. (* wtf ??? *)
+      iFrame "H1".
+    - unfold tpool_pointsto.
+      clear.
+      generalize (length σ).
+      intros p.
+      iInduction α as [| ??] "IH" forall (p).
+      + done.
+      + simpl.
+        rewrite big_opM_insert.
+        * iDestruct "H2" as "(H2 & H3)".
+          iSplitL "H2".
+          -- by iExists p.
+          -- iApply "IH".
+             iApply "H3".
+        * replace (S p) with (1 + p) by reflexivity.
+          assert (1 + p > p) as H; first lia.
+          revert H.
+          generalize (1 + p).
+          generalize p.
+          clear.
+          induction α as [| ? ? IH]; intros k p H.
+          -- done.
+          -- intros.
+             rewrite /= lookup_insert_ne; last lia.
+             apply IH; lia.
+  Admitted.
+
+  Lemma tpool_loc_dom l α tp :
+    own (tpool_name rs R) (to_tpool rs R tp)
+    -∗ tpool_pointsto l α -∗ ⌜is_Some (tp !! l)⌝.
+  Proof.
+    iIntros "Hinv Hloc".
+    iPoseProof (tpool_read with "Hinv Hloc") as "Hl".
+    destruct (tp !! l) ; eauto.
+    by rewrite option_equivI.
+  Qed.
+
+  Lemma tpool_write l α β σ :
+    own (tpool_name rs R) (to_tpool rs R σ)
+    -∗ tpool_pointsto l α
+    ==∗ own (tpool_name rs R) (●V <[l:=(to_agree (β))]>(to_tpool_go rs R 0 σ))
+      ∗ tpool_pointsto l β.
+  Proof.
+    iIntros "H Hl".
+    iMod (own_update_2 with "H Hl") as "[$ $]"; last done.
+    apply gmap_view_update.
+    intros.
+    split.
+    - admit.
+    - admit.
+  Admitted.
+
+  Lemma step_tick E j e :
+    nclose specN ⊆ E →
+    £ 1 ∗ spec_ctx ∗ ▷ j ⤇ Tick e ={E}=∗ j ⤇ e.
+  Proof.
+    iIntros (HSub) "[HCred [#HSpec HPt]]".
+    iDestruct "HSpec" as (tp σ) "HSpec".
+    iInv specN as "H" "HClose".
+    iApply (lc_fupd_add_later with "HCred").
+    iNext.
+    iDestruct "H" as (tp' σ' m) "[H [HS #HStep]]".
+    iAssert (⌜is_Some (tp' !! j)⌝)%I as "%Hdom".
+    { iApply (tpool_loc_dom with "H HPt"). }
+    destruct Hdom as [x Hx].
+    iAssert ((tp' !! j ≡ Some (Tick e)))%I as "#Hlookup".
+    { iApply (tpool_read with "H HPt"). }
+    iMod (tpool_write _ _ e with "H HPt") as "[Hh Hp]".
+    iMod ("HClose" with "[HS Hh]") as "_"; last by iModIntro.
+    iNext.
+    iExists (<[j:=e]> tp'), σ', (S m).
+    iFrame "HS".
+    iSplit; first last.
+    - iApply tp_internal_steps_many_L; last done.
+      unshelve epose proof (take_drop_middle tp' j x _) as H; first by rewrite Hx.
+      rewrite -H.
+      rewrite list_lookup_middle; first last.
+      {
+        rewrite length_take_le; first done.
+        eapply Nat.lt_le_incl, lookup_lt_Some; eassumption.
+      }
+      iDestruct (option_equivI with "Hlookup") as "G".
+      iRewrite "G".
+      iExists (take j tp'), (drop (S j) tp'), (Tick e), e, [].
+      iSplit; first done.
+      iSplit.
+      {
+        rewrite insert_app_r_alt; last (rewrite length_take; lia).
+        rewrite app_nil_r.
+        iApply f_equivI.
+        assert (j - length (take j tp') = 0) as ->.
+        {
+          rewrite length_take_le; first lia.
+          eapply Nat.lt_le_incl, lookup_lt_Some; eassumption.
+        }
+        simpl.
+        done.
+      }
+      iLeft.
+      done.
+    - rewrite /to_tpool /= /to_tpool'.
+      rewrite to_tpool_go_comm_insert; first done.
+      eapply lookup_lt_Some; eassumption.
+  Qed.
+
+  Lemma step_reify
+    `{subR : !subReifier sR rs}
+    E j
+    (op : opid (sReifier_ops sR))
+    (x : Ins (sReifier_ops sR op) ♯ IT)
+    (y : Outs (sReifier_ops sR op) ♯ IT)
+    (k : Outs (F (subEff_opid op)) ♯ IT -n> laterO IT)
+    (σ σ' : sReifier_state sR ♯ IT) β l :
+    nclose specN ⊆ E →
+    £ 1
+    ∗ sReifier_re sR op (x, σ) ≡ Some (y, σ', l)
+    ∗ k (subEff_outs y) ≡ Next β
+    ∗ spec_ctx
+    ∗ ▷ has_substate σ
+    ∗ ▷ j ⤇ (Vis (subEff_opid op) (subEff_ins x) k)
+    ={E}=∗ j ⤇ β
+         ∗ ([∗ list] i ∈ listO_map Tau l, ∃ j0 : natO, j0 ⤇ i)
+         ∗ has_substate σ'.
+  Proof.
+    iIntros (HSub) "(HCred & #Hr & #HEq & #HSpec & HSt & HPt)".
+    iDestruct "HSpec" as (tp σ'') "HSpec".
+    iInv specN as "H" "HClose".
+    iApply (lc_fupd_add_later with "HCred").
+    iNext.
+    iDestruct "H" as (tp' σ''' m) "[H [HS #HStep]]".
+    iAssert (⌜is_Some (tp' !! j)⌝)%I as "%Hdom".
+    { iApply (tpool_loc_dom with "H HPt"). }
+    destruct Hdom as [x' Hx].
+    iAssert ((tp' !! j ≡ Some (Vis (subEff_opid op) (subEff_ins x) k)))%I
+      as "#Hlookup".
+    { iApply (tpool_read with "H HPt"). }
+    iMod (tpool_write _ _ β
+           with "H HPt") as "[Hh Hp]".
+    iMod (tpool_alloc_big (listO_map Tau l) (<[j := β]>tp') with "[Hh]") as "[Hh Hpool]".
+    {
+      rewrite /to_tpool /to_tpool' /=.
+      rewrite to_tpool_go_comm_insert; first done.
+      apply lookup_lt_is_Some_1.
+      eexists _; eassumption.
+    }
+    destruct (gState_decomp sR_idx σ''') as [a rest] eqn:Hdecomp.
+    assert (σ''' ≡ gState_recomp rest a) as Hfs.
+    { symmetry. apply gState_recomp_decomp. by rewrite Hdecomp. }
+    iAssert (a ≡ (sR_state σ))%I with "[HS HSt]" as "#Hss".
+    {
+      iEval (rewrite Hfs) in "HS".
+      iApply (state_interp_has_state_idx_agree with "HS HSt").
+    }
+    iAssert (internal_step (gReifiers_sReifier rs)
+               ((Vis (subEff_opid op) (subEff_ins x) k)) σ'''
+               β (gState_recomp rest (sR_state σ')) (listO_map Tau l)) as "HStep'".
+    {
+      iRight.
+      iExists (subEff_opid op), (subEff_ins x), k.
+      iSplit; first done.
+      rewrite Tick_eq.
+      iDestruct (reify_vis_eqI_ctx_indep rs
+                     (subEff_opid op) (subEff_ins x) k
+                     (subEff_outs y) (gState_recomp rest (sR_state σ))
+                     (gState_recomp rest (sR_state σ')) l
+                  with "[]") as "Hreify".
+      {
+        iApply subReifier_reifyI_ctx_indep.
+        iApply "Hr".
+      }
+      iRewrite "HEq" in "Hreify".
+      setoid_replace σ''' with (gState_recomp rest a); last done.
+      iRewrite "Hss".
+      iApply "Hreify".
+    }
+    iEval (rewrite Hfs) in "HS".
+    iMod (state_interp_has_state_idx_update _ (sR_state σ') with "HS HSt") as "[HS HSt]".
+    iFrame "Hp Hpool HSt".
+    iApply "HClose".
+    iNext.
+    iExists (<[j := β]>tp' ++ (listO_map Tau l)),
+      (gState_recomp rest (sR_state σ')), (S m).
+    iSplitL "Hh".
+    - rewrite /to_tpool /to_tpool'.
+      rewrite -to_tpool_go_comm_union /=.
+      iFrame "Hh".
+    - iFrame "HS".
+      iApply tp_internal_steps_many_L; last done.
+      unshelve epose proof (take_drop_middle tp' j x' _) as H; first done.
+      rewrite -H; clear H.
+      rewrite list_lookup_middle; first last.
+      {
+        rewrite length_take_le; first done.
+        eapply Nat.lt_le_incl, lookup_lt_Some; eassumption.
+      }
+      iDestruct (option_equivI with "Hlookup") as "G".
+      iRewrite "G"; iClear "G".
+
+      iExists (take j tp'), (drop (S j) tp'), (Vis (subEff_opid op) (subEff_ins x) k), (β), (listO_map Tau l).
+      iSplit; first done.
+      iSplit.
+      {
+        rewrite insert_app_r_alt; last (rewrite length_take; lia).
+        rewrite -app_assoc.
+        iApply f_equivI.
+        assert (j - length (take j tp') = 0) as ->.
+        {
+          rewrite length_take_le; first lia.
+          eapply Nat.lt_le_incl, lookup_lt_Some; eassumption.
+        }
+        simpl.
+        done.
+      }
+      iApply "HStep'".
+  Qed.
+
+  Lemma step_reify_hom
+    `{subR : !subReifier sR rs}
+    (K : HOM) E j
+    (op : opid (sReifier_ops sR))
+    (x : Ins (sReifier_ops sR op) ♯ IT)
+    (y : Outs (sReifier_ops sR op) ♯ IT)
+    (k : Outs (F (subEff_opid op)) ♯ IT -n> laterO IT)
+    (σ σ' : sReifier_state sR ♯ IT) β l :
+    nclose specN ⊆ E →
+    £ 1
+    ∗ sReifier_re sR op (x, σ) ≡ Some (y, σ', l)
+    ∗ k (subEff_outs y) ≡ Next β
+    ∗ spec_ctx
+    ∗ ▷ has_substate σ
+    ∗ ▷ j ⤇ K (Vis (subEff_opid op) (subEff_ins x) k)
+    ={E}=∗ j ⤇ K β
+         ∗ ([∗ list] i ∈ listO_map Tau l, ∃ j0 : natO, j0 ⤇ i)
+         ∗ has_substate σ'.
+  Proof.
+    iIntros (HSub) "(HCred & #Hr & #HEq & #HSpec & HSt & HPt)".
+    rewrite hom_vis.
+    iDestruct (step_reify with "[Hr HEq $HSpec $HCred $HSt HPt]") as "H";
+      first done.
+    - iFrame "HPt".
+      iFrame "Hr".
+      rewrite /=.
+      iRewrite "HEq".
+      rewrite later_map_Next.
+      done.
+    - iApply "H".
+  Qed.
+
+  Lemma step_steps E j (e e' : IT) P σ σ' l m :
+    nclose specN ⊆ E →
+    ▷ P
+    ∗ £ 1
+    ∗ spec_ctx
+    ∗ ▷ has_full_state σ
+    ∗ internal_steps (gReifiers_sReifier rs) e σ e' σ' l m
+    ∗ ▷ j ⤇ e
+    ={E}=∗ P
+         ∗ j ⤇ e'
+         ∗ ([∗ list] i ∈ l, ∃ k : natO, k ⤇ i)
+         ∗ has_full_state σ'.
+  Proof.
+    iIntros (HSub) "(P & HCred & #Hspec & Hstate & #HSteps & HPt)".
+    iDestruct "Hspec" as (tp st) "Hspec".
+    iInv specN as "H" "HClose".
+    iApply (lc_fupd_add_later with "HCred").
+    iNext.
+    iDestruct "H" as (tp' st' p) "[H [HS #HSteps']]".
+    iAssert (⌜is_Some (tp' !! j)⌝)%I as "%Hdom".
+    { iApply (tpool_loc_dom with "H HPt"). }
+    destruct Hdom as [x' Hx].
+    iAssert ((tp' !! j ≡ Some e))%I
+      as "#Hlookup".
+    { iApply (tpool_read with "H HPt"). }
+    iAssert (st' ≡ σ)%I with "[HS Hstate]" as "#Hss".
+    { iApply (state_interp_has_full_state_agree with "HS Hstate"). }
+    iRewrite "Hss" in "HSteps'"; iRewrite "Hss" in "HS"; iRewrite "Hss" in "HClose";
+      iClear "Hss"; clear st'.
+    iAssert (e ≡ x')%I as "HEQ".
+    {
+      rewrite Hx.
+      iDestruct (internal_eq_sym with "Hlookup") as "Hlookup'".
+      iApply (option_equivI with "Hlookup'").
+    }
+    iRewrite "HEQ" in "HPt"; iRewrite "HEQ" in "HSteps";
+      iClear "Hlookup HEQ"; clear e.
+    iMod (tpool_write _ _ e' with "H HPt") as "[H HPt]".
+    iMod (tpool_alloc_big l (<[j := e']>tp') with "[H]") as "[H Hpool]".
+    {
+      rewrite /to_tpool /to_tpool' /=.
+      rewrite to_tpool_go_comm_insert; first done.
+      apply lookup_lt_is_Some_1.
+      eexists _; eassumption.
+    }
+    iMod (state_interp_has_full_state_update σ' with "HS Hstate")
+      as "[HS Hstate]".
+    iFrame "HPt Hpool Hstate P".
+    iApply "HClose".
+    iExists (<[j := e']>tp' ++ l), σ', (p + m).
+    iFrame "HS".
+    rewrite /to_tpool /to_tpool'.
+    rewrite -to_tpool_go_comm_union.
+    iFrame "H".
+    iNext.
+    unshelve epose proof (take_drop_middle tp' j x' _) as H; first done.
+    rewrite -H; clear H.
+    iPoseProof (internal_steps_tp_internal_steps with "HSteps") as "K".
+    iPoseProof (tp_internal_steps_trans with "K HSteps'") as "J".
+    iEval (rewrite Nat.add_comm).
+    iEval (rewrite insert_app_r_alt; last (rewrite length_take; lia)).
+    iEval (rewrite -app_assoc).
+    assert (j - length (take j tp') = 0) as ->.
+    {
+      rewrite length_take_le; first lia.
+      eapply Nat.lt_le_incl, lookup_lt_Some; eassumption.
+    }
+    iApply "J".
+  Qed.
+
+  Lemma step_steps_not_stateful P E j
+    (e e' : IT) l m :
+    nclose specN ⊆ E →
+    ▷ P
+    ∗ £ 1
+    ∗ spec_ctx
+    ∗ (∀ σ, internal_steps (gReifiers_sReifier rs) e σ e' σ l m)
+    ∗ ▷ j ⤇ e
+    ={E}=∗ P
+         ∗ j ⤇ e'
+         ∗ ([∗ list] i ∈ l, ∃ k : natO, k ⤇ i).
+  Proof.
+    iIntros (HSub) "(P & HCred & #Hspec & #HSteps & HPt)".
+    iDestruct "Hspec" as (tp st) "Hspec".
+    iInv specN as "H" "HClose".
+    iApply (lc_fupd_add_later with "HCred").
+    iNext.
+    iDestruct "H" as (tp' st' p) "[H [HS #HSteps']]".
+    iAssert (⌜is_Some (tp' !! j)⌝)%I as "%Hdom".
+    { iApply (tpool_loc_dom with "H HPt"). }
+    destruct Hdom as [x' Hx].
+    iAssert ((tp' !! j ≡ Some e))%I
+      as "#Hlookup".
+    { iApply (tpool_read with "H HPt"). }
+    iSpecialize ("HSteps" $! st').
+    iAssert (e ≡ x')%I as "HEQ".
+    {
+      rewrite Hx.
+      iDestruct (internal_eq_sym with "Hlookup") as "Hlookup'".
+      iApply (option_equivI with "Hlookup'").
+    }
+    iRewrite "HEQ" in "HPt"; iRewrite "HEQ" in "HSteps";
+      iClear "Hlookup HEQ"; clear e.
+    iMod (tpool_write _ _ e' with "H HPt") as "[H HPt]".
+    iMod (tpool_alloc_big l (<[j := e']>tp') with "[H]") as "[H Hpool]".
+    {
+      rewrite /to_tpool /to_tpool' /=.
+      rewrite to_tpool_go_comm_insert; first done.
+      apply lookup_lt_is_Some_1.
+      eexists _; eassumption.
+    }
+    iFrame "HPt Hpool P".
+    iApply "HClose".
+    iExists (<[j := e']>tp' ++ l), st', (p + m).
+    iFrame "HS".
+    rewrite /to_tpool /to_tpool'.
+    rewrite -to_tpool_go_comm_union.
+    iFrame "H".
+    iNext.
+    unshelve epose proof (take_drop_middle tp' j x' _) as H; first done.
+    rewrite -H; clear H.
+    iPoseProof (internal_steps_tp_internal_steps with "HSteps") as "K".
+    iPoseProof (tp_internal_steps_trans with "K HSteps'") as "J".
+    iEval (rewrite Nat.add_comm).
+    iEval (rewrite insert_app_r_alt; last (rewrite length_take; lia)).
+    iEval (rewrite -app_assoc).
+    assert (j - length (take j tp') = 0) as ->.
+    {
+      rewrite length_take_le; first lia.
+      eapply Nat.lt_le_incl, lookup_lt_Some; eassumption.
+    }
+    iApply "J".
+  Qed.
+
+End right_hand_side.
+
+Notation "j ⤇ e" := (tpool_pointsto _ _ j e) (at level 20) : bi_scope.
+
+Section rel.
+  Context {n : nat} (rs : gReifiers NotCtxDep n).
+  Notation F := (gReifiers_ops rs).
+  Context (R : ofe) `{!Cofe R}.
+  Notation IT := (IT F R).
+  Notation ITV := (ITV F R).
+  Context {Σ : gFunctors}.
+  Context `(HSTATE : !stateG rs R Σ).
+  Context `{!gitreeGS_gen rs R Σ} `{!tpoolSG rs R Σ}.
+  Notation iProp := (iProp Σ).
+  Notation coPsetO := (leibnizO coPset).
+  Context (s : stuckness).
+  Notation HOM := (@HOM R _ F).
+
+  Program Definition IT_Rel_pre
+    (IT_Val_Rel : ITV -n> ITV -n> iProp)
+    : IT -> IT -> iProp
+    := λ x y,
+      (∀ j (K : HOM), j ⤇ K y
+              -∗ WP@{rs} x @ s {{ v,
+                       ∃ v', j ⤇ K (IT_of_V v')
+                             ∗ IT_Val_Rel v v' }})%I.
+
+  Global Instance IT_Rel_pre_ne : NonExpansive3 IT_Rel_pre.
+  Proof.
+    intros ??? H1 ?? H2 ?? H3.
+    rewrite /IT_Rel_pre.
+    do 2 (f_equiv; intros ?).
+    f_equiv; first solve_proper.
+    f_equiv; first solve_proper.
+    intros ?; simpl.
+    f_equiv; intros ?.
+    f_equiv; solve_proper.
+  Qed.
+
+  Global Instance IT_Rel_pre_proper : Proper ((≡) ==> (≡) ==> (≡) ==> (≡)) IT_Rel_pre.
+  Proof.
+    intros ?? H1 ?? H2 ?? H3.
+    rewrite /IT_Rel_pre.
+    do 2 (f_equiv; intros ?).
+    f_equiv; first solve_proper.
+    f_equiv; first solve_proper.
+    intros ?; simpl.
+    f_equiv; intros ?.
+    f_equiv; solve_proper.
+  Qed.
+
+  Program Definition IT_Val_Rel_pre (R : ITV -n> ITV -n> iProp) :
+    ITV -n> ITV -n> iProp
+    := λne x y,
+      ((∃ a b, IT_of_V x ≡ core.Ret a
+               ∧ IT_of_V y ≡ core.Ret b
+               ∧ a ≡ b)
+       ∨ (∃ f g, IT_of_V x ≡ Fun f
+                 ∧ IT_of_V y ≡ Fun g
+                 ∧ □ ∀ v w,
+            ▷ (R v w
+               -∗ IT_Rel_pre R
+                    (APP' (IT_of_V x) (IT_of_V v))
+                    (APP' (IT_of_V y) (IT_of_V w)))))%I.
+  Next Obligation. solve_proper. Qed.
+  Next Obligation. solve_proper. Qed.
+
+  Global Instance IT_Val_Rel_pre_contractive : Contractive IT_Val_Rel_pre.
+  Proof.
+    intros m ?? H.
+    rewrite /IT_Val_Rel_pre.
+    intros ??; simpl.
+    do 4 f_equiv.
+    intros ?; simpl.
+    do 3 f_equiv.
+    do 2 (f_equiv; intros ?).
+    apply later_contractive.
+    destruct m as [| m].
+    - apply dist_later_0.
+    - apply dist_later_S.
+      f_equiv.
+      + apply dist_later_S in H.
+        solve_proper.
+      + do 1 (f_equiv; intros ?).
+        apply dist_later_S in H.
+        solve_proper.
+  Qed.
+
+  Program Definition IT_Val_Rel : ITV -n> ITV -n> iProp := fixpoint IT_Val_Rel_pre.
+
+  Lemma IT_Val_Rel_unfold' : IT_Val_Rel ≡ IT_Val_Rel_pre IT_Val_Rel.
+  Proof. apply fixpoint_unfold. Qed.
+
+  Program Definition IT_Rel := IT_Rel_pre IT_Val_Rel.
+
+  Lemma IT_Val_Rel_unfold v' w'
+    : IT_Val_Rel v' w' ≡
+        ((∃ a b, IT_of_V v' ≡ core.Ret a
+                 ∧ IT_of_V w' ≡ core.Ret b
+                 ∧ a ≡ b)
+         ∨ (∃ f g, IT_of_V v' ≡ Fun f
+                   ∧ IT_of_V w' ≡ Fun g
+                   ∧ □ ∀ v w,
+              ▷ (IT_Val_Rel v w
+                 -∗ IT_Rel
+                      (APP' (IT_of_V v') (IT_of_V v))
+                      (APP' (IT_of_V w') (IT_of_V w)))))%I.
+  Proof.
+    rewrite (IT_Val_Rel_unfold' v' w') /IT_Val_Rel_pre //=.
+  Qed.
+
+  Global Instance IT_Val_Rel_persist e1 e2 : Persistent (IT_Val_Rel e1 e2).
+  Proof.
+    rewrite IT_Val_Rel_unfold /IT_Val_Rel_pre.
+    apply _.
+  Qed.
+
+  Global Instance IT_Rel_proper : Proper ((≡) ==> (≡) ==> (≡)) IT_Rel.
+  Proof. solve_proper. Qed.
+
+  Global Instance IT_Rel_ne : NonExpansive2 IT_Rel.
+  Proof. solve_proper. Qed.
+
+  Global Instance IT_Val_Rel_proper1 : Proper ((≡) ==> (≡)) IT_Val_Rel.
+  Proof. solve_proper. Qed.
+
+  Global Instance IT_Val_Rel_proper2 a : Proper ((≡) ==> (≡)) (IT_Val_Rel a).
+  Proof. solve_proper. Qed.
+
+  Global Instance IT_Val_Rel_ne1 : NonExpansive IT_Val_Rel.
+  Proof. solve_proper. Qed.
+
+  Global Instance IT_Val_Rel_ne2 a : NonExpansive (IT_Val_Rel a).
+  Proof. solve_proper. Qed.
+
+  Definition IT_Top_Rel e1 e2 : iProp :=
+    spec_ctx rs _ HSTATE → IT_Rel e1 e2.
+
+  Global Instance IT_Top_Rel_proper : Proper ((≡) ==> (≡) ==> (≡)) IT_Top_Rel.
+  Proof. solve_proper. Qed.
+
+  Global Instance IT_Top_Rel_ne : NonExpansive2 IT_Top_Rel.
+  Proof. solve_proper. Qed.
+End rel.
+
+Notation "e1 ⪯ₑ e2 '@{' re \ A \ s '}'" :=
+  (IT_Rel re A s e1 e2) (at level 80) : bi_scope.
+Notation "e1 ⪯ᵥ e2 '@{' re \ A \ s '}'" :=
+  (IT_Val_Rel re A s e1 e2) (at level 80) : bi_scope.
+Notation "e1 ⪯ₚ e2 '@{' re \ A \ s \ H '}'" :=
+  (IT_Top_Rel re A H s e1 e2) (at level 80) : bi_scope.
+
+Lemma logrel_adequacy_internal Σ cr n
+  (rs : gReifiers NotCtxDep n)
+  {A} `{!Cofe A} `{!invGpreS Σ}
+  `{!Inhabited (gReifiers_state rs ♯ IT (sReifier_ops (gReifiers_sReifier rs)) A)}
+  `{!statePreG rs A Σ} `{!inG Σ (tpoolUR rs A)}
+  (α β : IT _ A) σ αv αs σ' (s : stuckness) k :
+
+  let rg := gReifiers_sReifier rs in
+  let F := sReifier_ops rg in
+  let IT := IT F A in
+  let ITV := ITV F A in
+
+  tp_external_steps rg [α] σ (IT_of_V αv :: αs) σ' k →
+  (∀ `{H1 : !gitreeGS_gen rs A Σ} `{!tpoolSG rs A Σ} `{HSTATE : !stateG rs A Σ},
+     (⊢@{iProp Σ} (£ cr
+                   -∗ @has_full_state _ _ rs _ _ _ HSTATE σ
+                   -∗ (α) ⪯ₚ (β) @{ rs \ A \ s \ HSTATE })%I)) →
+  ⊢@{iProp Σ} (∃ αv βs st' k', tp_internal_steps (gReifiers_sReifier rs) [β] σ
+                              (IT_of_V αv :: βs) st' k').
+Proof.
+  intros rg F IT' ITV' Hsteps Hprf.
+  unshelve eapply (step_fupdN_soundness_lc _ (S (weakestpre.steps_sum id 0 k))
+                     ((weakestpre.steps_sum id 0 k) + (S cr))).
+  {
+    (* TODO: plain instance for fixpoints *)
+    apply exist_plain. intros x1.
+    apply exist_plain. intros x2.
+    apply exist_plain. intros x3.
+    apply exist_plain. intros x4.
+    cut (∀ n α σ β σ', Plain (tp_internal_steps (Σ := Σ) (A := A)
+                                (gReifiers_sReifier rs) α σ β σ' n)).
+    { intros H; apply H. }
+    clear x1 x2 x3 x4.
+    intros x5.
+    induction x5 as [| ? IH]; intros x1 x2 x3 x4.
+    - rewrite tp_internal_steps_0.
+      apply _.
+    - rewrite tp_internal_steps_S.
+      apply exist_plain. intros y1.
+      apply exist_plain. intros y2.
+      apply and_plain.
+      + apply _.
+      + apply IH.
+  }
+  iIntros (H1) "(_HCred' & (_HCred & _HCred''))".
+  iMod (new_state_interp σ) as (H2) "[Hs Hs2]".
+  assert (G1 : (nat → ∀ σ, state_interp σ
+                           ⊢ |={∅}=> state_interp σ)).
+  { intros. iIntros "?". by iModIntro. }
+  assert (G2 : (nat → NonExpansive (λ σ, state_interp σ)%I)).
+  { solve_proper. }
+  assert (G3 : (nat → ∀ σ, state_interp σ
+                           ⊣⊢ True ∗ state_interp σ)).
+  {
+    intros. iSplit; iIntros "H".
+    - by iFrame "H".
+    - by iDestruct "H" as "(_ & ?)".
+  }
+  pose GGS : gitreeGS_gen rs A Σ :=
+    GitreeG rs A Σ H1 H2
+      (λ n σ, @state_interp _ _ rs A _ _ H2 σ)%I
+      (λ _, True%I)
+      (λ _, True%I)
+      ltac:(solve_proper)
+      id
+      G1
+      G2
+      G3.
+  iMod (new_state_interp σ) as (sg') "[Hs' Hsfull']".
+  iMod (own_alloc ((to_tpool rs A []))) as (γ) "Ht".
+  { by apply gmap_view_auth_dfrac_valid. }
+  set (T := {| tpool_inG := _; tpool_name := γ |} : tpoolSG rs A Σ).
+  iPoseProof (Hprf GGS T sg') as "#H". clear Hprf.
+  iDestruct (tp_external_steps_tp_internal_steps _ _ _ _ _ _ Hsteps) as "Hsteps".
+  iSpecialize ("H" with "_HCred'' Hsfull'").
+  iMod (tpool_alloc rs A β 0 with "[$Ht]") as "(Ht & Hp)"; first done.
+  iMod (inv_alloc specN _ (spec_inv rs A sg' [β] σ)
+         with "[Hs' Ht]") as "#Hinv".
+  {
+    iNext.
+    unfold spec_inv.
+    iExists [β], σ, 0.
+    iFrame "Ht Hs'".
+    by iApply tp_internal_steps_0.
+  }
+  iAssert (spec_ctx rs A sg') with "[]" as "G".
+  { iExists [β], σ. iFrame "Hinv". }
+  iSpecialize ("H" with "G").
+  iSpecialize ("H" $! 0 HOM_id with "Hp").
+  set (Φs := [(λ v, ∃ v', (0 ⤇ idfun (IT_of_V v')
+                           ∗ IT_Val_Rel _ _ s v v') ∗ £ 1)%I]).
+  assert (Forall (λ f : ITV (sReifier_ops (gReifiers_sReifier rs)) A → iProp Σ,
+                NonExpansive f) Φs) as HEΦs.
+  {
+    apply Forall_singleton.
+    solve_proper_prepare.
+    f_equiv. intros ?; simpl.
+    f_equiv. f_equiv. f_equiv.
+    f_equiv.
+    done.
+  }
+  iMod (wptp_postconditions
+                rs Φs HEΦs s k _ _ _ 0 _
+              with "Hsteps [Hs] [_HCred'] [H _HCred]") as "J".
+  { iSimpl. iApply "Hs". }
+  { iSimpl. iApply "_HCred'". }
+  {
+    rewrite /wptp big_sepL2_singleton.
+    iApply (wp_wand with "H").
+    iIntros (v) "_G".
+    iModIntro.
+    iDestruct "_G" as (v') "_G".
+    iExists v'.
+    iFrame "_G _HCred".
+  }
+  rewrite step_fupdN_S_fupd.
+  iModIntro.
+  iApply (step_fupdN_wand with "J").
+  iModIntro. iNext. iModIntro.
+  iIntros "J".
+  iMod "J".
+  subst Φs.
+  iSimpl in "J".
+  iDestruct "J" as (nt') "(HS & H1 & _)".
+  match goal with
+  | |- context G [from_option ?a] =>
+      set (Φ := a)
+  end.
+  iDestruct (internal_eq_rewrite (IT_to_V (IT_of_V αv))
+               (Some αv)
+               (from_option Φ True%I) with "[] H1") as "H1".
+  { subst Φ. solve_proper. }
+  { iPureIntro. rewrite IT_to_of_V. done. }
+  subst Φ. iSimpl in "H1".
+  iDestruct "H1" as (v') "((Hpt & Hrel) & HCred)".
+  iInv specN as (tp σ'' m) "(J1 & J2 & #J3)" "HClose".
+  iClear "Hinv G".
+  iApply (lc_fupd_add_later with "HCred").
+  iNext.
+  iPoseProof (tpool_loc_dom with "J1 Hpt") as "%K".
+  iAssert (⌜∃ αv βs, tp ≡ IT_of_V αv :: βs⌝)%I with "[J1 Hpt]" as "%K'".
+  {
+    iPoseProof (tpool_read with "J1 Hpt") as "K".
+    destruct tp as [| o tp'].
+    - exfalso.
+      destruct K as [? K].
+      inversion K.
+    - iSimpl in "K".
+      iDestruct (option_equivI with "K") as "K".
+      destruct v'.
+      + iSimpl in "K".
+        iDestruct (ret_discrete_pure' (gReifiers_sReifier rs) o o0 with "K") as (β') "%J".
+        iExists (core.RetV β'), tp'.
+        iPureIntro. simpl.
+        by rewrite J.
+      + iSimpl in "K".
+        iDestruct (fun_discrete_pure' (gReifiers_sReifier rs) o o0 with "K") as (β') "%J".
+        iExists (core.FunV β'), tp'.
+        iPureIntro. simpl.
+        by rewrite J.
+  }
+  destruct K' as [? [? HEQ]].
+  iAssert (▷ spec_inv rs A sg' [β] σ)%I with "[J2 J1]" as "JJJ".
+  {
+    iNext.
+    unfold spec_inv.
+    iExists tp, σ'', m.
+    iFrame "J3 J2 J1".
+  }
+  iSpecialize ("HClose" with "JJJ").
+  iMod "HClose".
+  iAssert (tp_internal_steps (gReifiers_sReifier rs) [β] σ
+             (IT_of_V x :: x0) σ'' m)%I as "J3'".
+  {
+    rewrite /tp_internal_steps /=.
+    by rewrite -HEQ.
+  }
+  iApply fupd_mask_intro; first done.
+  iIntros "_".
+  iExists x, x0, σ'', m.
+  iFrame "J3'".
+Qed.
+
+Lemma logrel_adequacy `{Classical} Σ cr n
+  (rs : gReifiers NotCtxDep n)
+  {A} `{!Cofe A} `{!invGpreS Σ}
+  `{!Inhabited (gReifiers_state rs ♯ IT (sReifier_ops (gReifiers_sReifier rs)) A)}
+  `{!statePreG rs A Σ} `{!inG Σ (tpoolUR rs A)}
+  (α β : IT _ A) σ αv αs σ' (s : stuckness) k :
+
+  let rg := gReifiers_sReifier rs in
+  let F := sReifier_ops rg in
+  let IT := IT F A in
+  let ITV := ITV F A in
+
+  tp_external_steps rg [α] σ (IT_of_V αv :: αs) σ' k →
+  (∀ `{H1 : !gitreeGS_gen rs A Σ} `{!tpoolSG rs A Σ} `{HSTATE : !stateG rs A Σ},
+     (⊢@{iProp Σ} (£ cr
+                   -∗ @has_full_state _ _ rs _ _ _ HSTATE σ
+                   -∗ (α) ⪯ₚ (β) @{ rs \ A \ s \ HSTATE })%I)) →
+  (∃ αv βs st' k', tp_external_steps (gReifiers_sReifier rs) [β] σ
+                     (IT_of_V αv :: βs) st' k').
+Proof.
+  intros rg ops IT ITV Hsteps Hwp.
+  epose proof (logrel_adequacy_internal Σ cr n rs α β σ αv αs σ' s k Hsteps Hwp) as J.
+
+  epose proof (@tp_internal_steps_safe_agnostic A _ NotCtxDep rg Σ _ [β] σ).
+
+Section rules.
+  Context {n : nat} (rs : gReifiers NotCtxDep n).
+  Notation F := (gReifiers_ops rs).
+  Context (R : ofe) `{!Cofe R}.
+  Notation IT := (IT F R).
+  Notation ITV := (ITV F R).
+  Context `{!gitreeGS_gen rs R Σ} `{!tpoolSG rs R Σ}.
+  Notation iProp := (iProp Σ).
+  Notation coPsetO := (leibnizO coPset).
+  Context (s : stuckness).
+  Notation HOM := (@HOM R _ F).
+
+  Lemma IT_Rel_val `{!IntoVal e1 v} `{!IntoVal e2 w}
+    : ⊢ (v) ⪯ᵥ (w) @{ rs \ R \ s }
+        -∗ (e1) ⪯ₑ (e2) @{ rs \ R \ s }.
+  Proof.
+    iIntros "H".
+    rewrite -(@into_val _ _ _ e1) -(@into_val _ _ _ e2).
+    iIntros (j K) "Hpt".
+    iApply wp_val.
+    iModIntro.
+    iExists w.
+    iFrame "Hpt H".
+  Qed.
+
+  Lemma IT_Rel_Tick_l' e1 e2
+    : ⊢ ▷ (£ 1 -∗ (e1) ⪯ₑ (e2) @{ rs \ R \ s })
+        -∗ (Tick e1) ⪯ₑ (e2) @{ rs \ R \ s }.
+  Proof.
+    iIntros "H" (j K) "G".
+    iApply wp_tick.
+    iNext.
+    iIntros "Hlc".
+    by iApply ("H" with "Hlc").
+  Qed.
+
+  Lemma IT_Rel_Tick_l `{HSTATE : !stateG rs R Σ} e1 e2
+    : ⊢ ▷ (£ 1 -∗ (e1) ⪯ₚ (e2) @{ rs \ R \ s \ HSTATE })
+        -∗ (Tick e1) ⪯ₚ (e2) @{ rs \ R \ s \ HSTATE }.
+  Proof.
+    iIntros "H HInv".
+    iApply IT_Rel_Tick_l'.
+    iNext.
+    iIntros "Hlc".
+    iApply ("H" with "Hlc HInv").
+  Qed.
+
+  Lemma IT_Rel_Tick_r
+    `{HSTATE : !stateG rs R Σ} e1 e2
+    : ⊢ £ 1 -∗ (e1) ⪯ₚ (e2) @{ rs \ R \ s \ HSTATE }
+        -∗ e1 ⪯ₚ (Tick e2) @{ rs \ R \ s \ HSTATE }.
+  Proof.
+    iIntros "HCred H #HInv %j %K G".
+    iApply fupd_wp; first solve_proper.
+    iEval (rewrite hom_tick) in "G".
+    iMod (step_tick with "[$HCred $HInv $G]") as "J";
+      first set_solver.
+    iModIntro.
+    iSpecialize ("H" with "HInv").
+    iApply ("H" $! j K with "J").
+  Qed.
+
+  Lemma IT_Rel_Tick_lr
+    `{HSTATE : !stateG rs R Σ} e1 e2
+    : ⊢ (e1) ⪯ₚ (e2) @{ rs \ R \ s \ HSTATE }
+        -∗ (Tick e1) ⪯ₚ (Tick e2) @{ rs \ R \ s \ HSTATE }.
+  Proof.
+    iIntros "H".
+    iApply IT_Rel_Tick_l.
+    iNext.
+    iIntros "Hlc".
+    iApply (IT_Rel_Tick_r with "Hlc H").
+  Qed.
+
+  Lemma IT_Rel_bottom_l' e
+    : ⊢ (core.Bottom) ⪯ₑ (e) @{ rs \ R \ s }.
+  Proof.
+    iLöb as "IH".
+    iEval (rewrite Bottom_unfold -Tick_eq).
+    iApply IT_Rel_Tick_l'.
+    iNext.
+    by iIntros "_".
+  Qed.
+
+  Lemma IT_Rel_bottom_l `{HSTATE : !stateG rs R Σ} e
+    : ⊢ (core.Bottom) ⪯ₚ (e) @{ rs \ R \ s \ HSTATE }.
+  Proof.
+    iIntros "HInv".
+    iApply IT_Rel_bottom_l'.
+  Qed.
+
+  Lemma IT_Rel_Vis_l
+    `{subR : !subReifier sR rs}
+    (op : opid (sReifier_ops sR))
+    (x : Ins (sReifier_ops sR op) ♯ IT)
+    (y : Outs (sReifier_ops sR op) ♯ IT)
+    (k : Outs (F (subEff_opid op)) ♯ IT -n> laterO IT)
+    (σ σ' : sReifier_state sR ♯ IT) β l e :
+    sReifier_re sR op (x, σ) ≡ Some (y, σ', l) →
+    k (subEff_outs y) ≡ Next β →
+    has_substate σ
+    -∗ ▷ (£ 1 -∗ has_substate σ'
+          -∗ (wptp rs s (listO_map Tau l) (replicate (length (listO_map Tau l)) fork_post))
+          ∗ (β) ⪯ₑ (e) @{ rs \ R \ s})
+    -∗ (Vis (subEff_opid op) (subEff_ins x) k) ⪯ₑ (e) @{ rs \ R \ s}.
+  Proof.
+    iIntros (H1 H2) "Hσ G".
+    iIntros (j K) "J".
+    iApply (wp_subreify_ctx_indep with "Hσ"); [eassumption | eassumption |].
+    iNext.
+    iIntros "Hlc Hσ".
+    iDestruct ("G" with "Hlc Hσ") as "(G1 & G2)".
+    iFrame "G1".
+    by iApply "G2".
+  Qed.
+
+  Lemma IT_Rel_Vis_r
+    `(HSTATE : !stateG rs R Σ)
+    `{subR : !subReifier sR rs}
+    e
+    (op : opid (sReifier_ops sR))
+    (x : Ins (sReifier_ops sR op) ♯ IT)
+    (y : Outs (sReifier_ops sR op) ♯ IT)
+    (k : Outs (F (subEff_opid op)) ♯ IT -n> laterO IT)
+    (σ σ' : sReifier_state sR ♯ IT) β l
+    : £ 1
+      -∗ sReifier_re sR op (x, σ) ≡ Some (y, σ', l)
+      -∗ k (subEff_outs y) ≡ Next β
+      -∗ ▷ has_substate σ
+      -∗ (([∗ list] i ∈ listO_map Tau l, ∃ j0 : natO, j0 ⤇ i)
+          -∗ has_substate σ'
+          -∗ (e) ⪯ₚ (β) @{ rs \ R \ s \ HSTATE })
+      -∗ (e) ⪯ₚ (Vis (subEff_opid op) (subEff_ins x) k) @{ rs \ R \ s \ HSTATE }.
+  Proof.
+    iIntros "HCred Heq1 Heq2 Hst H #HInv %j %K G".
+    iApply fupd_wp; first solve_proper.
+    iMod (step_reify_hom with "[$HCred $Heq1 $Heq2 $Hst $HInv $G]")
+      as "(J1 & J2 & J3)";
+      first set_solver.
+    iModIntro.
+    iApply ("H" with "J2 J3 HInv J1").
+  Qed.
+
+End rules.
+
+Require Import gitrees.gitree.subofe.
+Require Import gitrees.gitree.lambda.
+Require Import gitrees.effects.store.
+Require Import gitrees.lib.factorial.
+
+Section example.
+  Context {n : nat} (rs : gReifiers NotCtxDep n).
+  Notation F := (gReifiers_ops rs).
+  Context `{!subReifier reify_store rs}.
+  Context (R : ofe) `{!Cofe R}.
+  Context `{!SubOfe natO R, !SubOfe unitO R}.
+  Notation IT := (IT F R).
+  Notation ITV := (ITV F R).
+  Context `{!gitreeGS_gen rs R Σ}.
+  Context `{!tpoolSG rs R Σ} `{!heapG rs R Σ}.
+  Context `{HSTATE : !stateG rs R Σ}.
+  Notation iProp := (iProp Σ).
+  Notation coPsetO := (leibnizO coPset).
+  Context (s : stuckness).
+  Notation HOM := (@HOM R _ F).
+
+  Example prog3 : ITV := FunV (Next (λne x, x)).
+
+  Program Example prog4 : IT := λit x, LET (Ret 5) (constO x).
+  Next Obligation.
+    intros ??? G.
+    by do 2 f_equiv.
+  Qed.
+
+  Program Example prog5 : IT := λit x, ALLOC (Ret 5) (constO x).
+  Next Obligation.
+    intros ??? H.
+    by do 2 f_equiv.
+  Qed.
+
+  Program Example prog6 : IT := (IT_of_V prog3) ⊙ (IT_of_V prog3).
+
+  (* do reverse *)
+  Example prog3_prog4_rel
+    : ⊢ (IT_of_V prog3) ⪯ₚ (prog4) @{ rs \ R \ s \ HSTATE }.
+  Proof.
+    iIntros "#HInv".
+    iApply IT_Rel_val.
+    rewrite IT_Val_Rel_unfold.
+    iRight.
+    iExists (Next (λne x, x)), _.
+    iSplit; first done.
+    iSplit; first done.
+    iModIntro.
+    iIntros (v w).
+    iNext.
+    iIntros "H".
+    iEval (rewrite !APP'_Fun_l /= -!Tick_eq LET_Val /=).
+    iApply (IT_Rel_Tick_lr with "[H] HInv").
+    iIntros "_".
+    iApply IT_Rel_val.
+    iApply "H".
+  Qed.
+
+  Example prog4_prog3_rel
+    : ⊢ (prog4) ⪯ₚ (IT_of_V prog3) @{ rs \ R \ s \ HSTATE }.
+  Proof.
+    iIntros "#HInv".
+    iApply IT_Rel_val.
+    rewrite IT_Val_Rel_unfold.
+    iRight.
+    iExists _, _.
+    iSplit; first done.
+    iSplit; first done.
+    iModIntro.
+    iIntros (v w).
+    iNext.
+    iIntros "H".
+    iEval (rewrite !APP'_Fun_l /= -!Tick_eq LET_Val /=).
+    iApply (IT_Rel_Tick_lr with "[H] HInv").
+    iIntros "_".
+    iApply IT_Rel_val.
+    iApply "H".
+  Qed.
+
+  Example prog5_prog3_rel
+    : heap_ctx rs
+      -∗ (prog5) ⪯ₚ (IT_of_V prog3) @{ rs \ R \ s \ HSTATE }.
+  Proof.
+    iIntros "#HHeap #HInv".
+    iApply IT_Rel_val.
+    rewrite IT_Val_Rel_unfold.
+    iRight.
+    iExists _, (Next (λne x, x)).
+    iSplit; first done.
+    iSplit; first done.
+    iModIntro.
+    iIntros (v w).
+    iNext.
+    iIntros "#H".
+    iEval (rewrite !APP'_Fun_l /= -!Tick_eq).
+    iApply (IT_Rel_Tick_l with "[H] HInv").
+    iNext.
+    iIntros "Hlc _ %j %K Hpt".
+    iApply (wp_alloc with "HHeap"); first solve_proper.
+    do 2 iNext.
+    iIntros (l) "Hpt'"; iSimpl.
+    iApply wp_val.
+    iMod (step_steps_not_stateful _ _ _ emp%I _ _ _ (K (IT_of_V w)) [] 1
+           with "[$Hlc $HInv $Hpt]") as "(_ & J & _)";
+      first set_solver.
+    {
+      iSplit; first done.
+      iIntros (σ).
+      iApply internal_steps_S.
+      iExists _, _, [], [].
+      iSplit; [done | iSplit]; last (iApply internal_steps_0; by iSplit).
+      iLeft.
+      rewrite hom_tick.
+      by iSplit.
+    }
+    iModIntro.
+    iExists w.
+    by iFrame "H J".
+  Qed.
+
+  Program Definition heap_ctx_rel :=
+    inv stateN
+      (∃ σ rest, @has_full_state _ _ rs _ _ _ HSTATE
+                   (gState_recomp rest (sR_state σ))
+            ∗ own (heapG_name rs) (●V (fmap (M := gmap locO) to_agree σ)))%I.
+
+  Example prog5_prog5_rel
+    `{!Inhabited (gState_rest sR_idx rs ♯
+                    ITF_solution.IT (sReifier_ops (gReifiers_sReifier rs)) R)}
+    : heap_ctx rs -∗ heap_ctx_rel
+      -∗ (prog5) ⪯ₚ (prog5) @{ rs \ R \ s \ HSTATE }.
+  Proof.
+    iIntros "#HHeap #HHeap' #HInv".
+    iApply IT_Rel_val.
+    rewrite IT_Val_Rel_unfold.
+    iRight.
+    iExists _, _.
+    iSplit; first done.
+    iSplit; first done.
+    iModIntro.
+    iIntros (v w).
+    iNext.
+    iIntros "#H".
+    iEval (rewrite !APP'_Fun_l /= -!Tick_eq).
+    iApply (IT_Rel_Tick_l with "[H] HInv").
+    iNext. iIntros "Hlc".
+    iIntros "_ %j %K Hpt".
+
+    iApply (wp_alloc with "HHeap"); first solve_proper.
+    do 2 iNext.
+    iIntros (l) "Hpt'".
+    iSimpl.
+    iApply wp_val.
+    iExists w.
+    iFrame "H".
+
+    iInv "HHeap'" as "(%σ & %rest & Hstate & Hheap)" "Hcl".
+    set (l' := (Loc.fresh (dom σ))).
+    iMod (step_steps with "[$Hheap $Hlc $HInv $Hstate $Hpt]")
+      as "(J1 & J2 & J3 & J4)".
+    {
+      rewrite /specN /stateN.
+      apply namespaces.coPset_subseteq_difference_r; last done.
+      apply ndot_ne_disjoint.
+      done.
+    }
+    {
+      iApply internal_steps_S.
+      iExists _, (gState_recomp rest (sR_state σ)), [], []. iSplit; first done.
+      iSplit.
+      { iApply internal_step_hom. iLeft. iSplit; done. }
+      iApply internal_steps_S.
+
+      iExists (K (IT_of_V w)),
+        (gState_recomp rest (sR_state (<[l' := Next (Ret 5)]>σ))),
+        [], []. iSplit; first done.
+      iSplit.
+      {
+        iApply internal_step_hom. iRight. iExists _, _, _. iSplit; first done.
+        iEval (rewrite Tick_eq).
+        simplify_eq; cbn-[gState_recomp].
+        rewrite (reify_vis_eq_ctx_indep _ _ _ _ _ _ _ []) //; first last.
+        {
+          eapply (@subReifier_reify _ NotCtxDep reify_store rs _ IT _
+                    (inr (inr (inl ())))
+                    (1, Next (Ret 5)) _ σ
+                    (<[l':=Next (Ret 5)]> σ) rest []).
+          simpl.
+          rewrite Loc.add_0.
+          subst l'.
+          rewrite insert_empty -insert_union_singleton_l.
+          reflexivity.
+        }
+      }
+      iApply internal_steps_0.
+      iSplit; done.
+    }
+    iMod (istate_alloc _ (Ret 5) l' with "J1") as "(T1 & T2)".
+    {
+      apply (not_elem_of_dom_1 (M:=gmap loc)).
+      subst l'.
+      rewrite dom_fmap_L.
+      rewrite -(Loc.add_0 (Loc.fresh (dom σ))).
+      apply Loc.fresh_fresh. lia.
+    }
+    iClear "J3".
+    iFrame "J2".
+
+    iApply ("Hcl" with "[J4 T1]").
+    iNext.
+    iExists _, _; iFrame "J4".
+    rewrite -(fmap_insert to_agree σ).
+    iFrame "T1".
+  Qed.
+
+End example.
+
+(* Inductive class : (IT -> IT) -> Prop := *)
+(* | id : class idfun *)
+(* | comp f g : class f -> class g -> class (compose f g) *)
+(* | tricky (C' : IT -> IT -n> IT) : (∀ x, class (C' x)) -> class (λ x, Fun (Next (C' x))). *)
